module graph functions changed according to discussion with Keyin

src/ModuleGraph_simplified.v
@@ -9,7 +9,18 @@ From mathcomp Require Import ssreflect ssrbool ssrnat eqtype seq fintype.
    (mainly registers, wires, ports, nodes) in the graph,
    but instead of edges have expressions. *)
 
-(* Type of vertices of a module graph *)
+
+
+
+(*****************************************************************************)
+(*                                                                           *)
+(*                          M O D U L E   G R A P H S                        *)
+(*                                                                           *)
+(*****************************************************************************)
+
+
+(*---------------------------------------------------------------------------*)
+(* Vertices                                                                  *)
 
 Inductive vertex_type :=
    (* what kind of vertices can be in the module graph *)
@@ -118,16 +129,22 @@ Definition output_connectors (v : vertex_type) : seq fgtyp :=
 
 (* vertex set of a module graph (using pairs of natural numbers as keys) *)
 
-Module MakeVtypFMap (V : SsrOrder) (VM : SsrFMapWithNew with Module SE := V)
-<: SsrFMapWithNew with Module SE := V.
+Module MakeVtypFMap (V : SsrOrder) (VM : SsrFMap with Module SE := V)
+<: SsrFMap with Module SE := V.
   Include VM.
   Include FMapLemmas VM.
   Definition env : Type := t vertex_type.
 End MakeVtypFMap.
 
-Module ProdVarOrder := MakeProdOrderWithDefaultSucc VarOrder VarOrder.
-Module PVM <: SsrFMapWithNew := FMaps.MakeTreeMapWithNew ProdVarOrder.
-Module module_graph_vertex_set_p <: SsrFMapWithNew := MakeVtypFMap ProdVarOrder PVM.
+Module ProdVarOrder := MakeProdOrder VarOrder VarOrder.
+Module PVM <: SsrFMap := FMaps.MakeTreeMap ProdVarOrder.
+Module module_graph_vertex_set_p <: SsrFMap := MakeVtypFMap ProdVarOrder PVM.
+
+
+
+
+(*---------------------------------------------------------------------------*)
+(* Connection expressions                                                    *)
 
 (* connections of a module graph:
    For every input connector of a module graph, there should be an associated expression.
@@ -175,7 +192,7 @@ Canonical def_expr_eqType := Eval hnf in EqType def_expr def_expr_eqMixin.
 
 (* for connection_tree, whose key is (N_pair, N) as input_connector_id
    here this module produce ProdOrder like ((N,N),N) *)
-Module MakeProdOrderWithDefaultSucc2 (O1 O2 : SsrOrderWithDefaultSucc) <: SsrOrderWithDefaultSucc
+(*Module MakeProdOrderWithDefaultSucc2 (O1 O2 : SsrOrderWithDefaultSucc) <: SsrOrderWithDefaultSucc
     with Definition T := prod_eqType O1.T O2.T.
   Module M := MakeProdOrderMinimal O1 O2.
   Module P := MakeSsrOrder M.
@@ -187,313 +204,52 @@ Module MakeProdOrderWithDefaultSucc2 (O1 O2 : SsrOrderWithDefaultSucc) <: SsrOrd
     case: x => x y. rewrite /ltn /succ /=. rewrite /M.ltn /=.
     rewrite O2.ltn_succ andbT eqtype.eq_refl orbT //.
   Qed.
-End MakeProdOrderWithDefaultSucc2.
+End MakeProdOrderWithDefaultSucc2.*)
 
 (* can be identifier of a input/output_connector *)
-Module PProdVarOrder := MakeProdOrderWithDefaultSucc2 ProdVarOrder VarOrder.
+Module PProdVarOrder := MakeProdOrder ProdVarOrder VarOrder.
 
-Module MakeCnctFMap (V : SsrOrder) (VM : SsrFMapWithNew with Module SE := V)
-<: SsrFMapWithNew with Module SE := V.
+Module MakeCnctFMap (V : SsrOrder) (VM : SsrFMap with Module SE := V)
+<: SsrFMap with Module SE := V.
   Include VM.
   Include FMapLemmas VM.
   Definition env : Type := t def_expr.
 End MakeCnctFMap.
 
-Module PPVM <: SsrFMapWithNew := FMaps.MakeTreeMapWithNew PProdVarOrder.
-Module module_graph_connection_trees_p <: SsrFMapWithNew := MakeCnctFMap PProdVarOrder PPVM.
+Module PPVM <: SsrFMap := FMaps.MakeTreeMap PProdVarOrder.
+Module module_graph_connection_trees_p <: SsrFMap := MakeCnctFMap PProdVarOrder PPVM.
 
-(* Semantics.
-   In a module graph, identifiers of vertices are pairs of natural numbers.
-   These numbers come from Sreg, Swire etc. statements.
-   The pair satisfies this condition:
-   if the type of the vertex is aggregate, then the pair has the form (v, 0);
-   also, there is no other identifier used in the module of the form (v, w) (for any number w). *)
 
-(* type of a tmap, which records the aggr_type for each element *)
-Definition ft_pmap := (N*N) -> (option ftype).
-Definition ft_find (v : N*N) (m : ft_pmap) := m v.
-Definition ft_add (v : N*N) (ft : ftype) (m : ft_pmap) : ft_pmap :=
-   fun (y : N*N) => if y == v then (Some ft) else (ft_find y m).
-Definition ft_mem (v : N*N) (m : ft_pmap) : bool := if (m v == None) then false else true.
-Definition ft_empty : ft_pmap := (fun _ => None).
 
-Fixpoint select_field (f : VarOrder.t) (l : seq PProdVarOrder.t) (ff : ffield) : option (seq PProdVarOrder.t * ftype) :=
-(* select field f from the list of input connectors l, which corresponds to type ff.
-   ff does not need to be passive, but its direction is ignored.
-   Return the corresponding output connectors, and also return the type of the field f. *)
-match ff with
-| Fflips v _ ft ff' =>
-    let elsize := size_of_ftype ft in
-    if size l < elsize then None
-    else if f == v then Some (take elsize l, ft)
-         else select_field f (drop elsize l) ff'
-| _ => None
-end.
 
-Fixpoint list_lhs_ref_p (ref : HiFP.href) (tmap : ft_pmap) : option (seq PProdVarOrder.t * ftype) :=
-(* find which input connectors of ground-type identifiers correspond to reference ref.
-   ground-type identifiers are vertices in the module graph (identified by a pair of N);
-   output connectors are always the triple (vertex identifier, N0).
-   Also find the type of expression e. *)
-match ref with
-| Eid v =>
-    (* Construct a list of identifiers and find the type of v *)
-    match tmap v with
-    | Some (Gtyp gt) => Some ([:: (v, N0)], Gtyp gt)
-    | Some t =>
-        if snd v == N0
-        then Some (mkseq (fun i => (fst v, N.of_nat (i + 1), N0)) (size_of_ftype t), t)
-        else None
-    | None => None
-    end
-| Esubfield ref' f =>
-    match list_lhs_ref_p ref' tmap with
-    | Some (l, Btyp ff) =>
-        (* Select from list l the relevant part for field f.
-           Determine which part this is based on t *)
-        select_field f l ff
-    | _ => None
-    end
-| Esubindex ref' n =>
-    match list_lhs_ref_p ref' tmap with
-    | Some (l, Atyp t m) =>
-        (* Select from list l the relevant part for array element n.
-           Determine which part this is based on t *)
-        let elsize := size_of_ftype t in
-        if (n < m) && (size l == m * elsize)
-        then Some (take elsize (drop (n * elsize) l), t)
-        else None
-    | _ => None
-    end
-| Esubaccess _ _ => None
-end.
+(*****************************************************************************)
+(*                                                                           *)
+(*             E X P R E S S I O N S   A N D   T Y P E   M A P S             *)
+(*                                                                           *)
+(*****************************************************************************)
 
-(* Semantics: *)
 
-Definition connect_non_passive_fgtyp (ct_old : module_graph_connection_trees_p.env)
-                                     (_ : HiFP.href) (lst_tgt : list PProdVarOrder.t) (gt_tgt : fgtyp)
-                                     (ref_src : HiFP.href) (lst_src : list PProdVarOrder.t) (gt_src : fgtyp)
-                                     (ct_new : module_graph_connection_trees_p.env) : bool :=
-(* The predicate checks whether ct_new contains the correct connection that connects from lst_src to lst_tgt,
-   and it does not change the connection into lst_src.
-   These lists must be one-element lists for output and input connectors of compatible types. *)
-      match lst_tgt, lst_src with
-      | [:: ic], [:: oc] =>    (module_graph_connection_trees_p.find ic ct_new == Some (D_fexpr (Eref ref_src)))
-                            &&
-                               (module_graph_connection_trees_p.find oc ct_new == module_graph_connection_trees_p.find oc ct_old)
-                               (* why this is compared?
-                                  In Sem_frag_stmt, it is ensured that connection trees NOT related to tgt or src are not changed.
-                                  Here, we need to ensure that the connection tree of tgt is changed
-                                  and the connection tree of src remains the same. *)
-      | _, _ => false
-      end
-   &&
-      match gt_tgt, gt_src with
-      | Fuint _, Fuint _
-      | Fuint _, Fuint_implicit _
-      | Fsint _, Fsint _
-      | Fsint _, Fsint_implicit _
-      | Fclock, Fclock
-      | Fasyncreset, Fasyncreset => true
-      | Fuint_implicit wt, Fuint ws
-      | Fuint_implicit wt, Fuint_implicit ws
-      | Fsint_implicit wt, Fsint ws
-      | Fsint_implicit wt, Fsint_implicit ws => wt >= ws
-      | _, _ => false
-      end.
+(*---------------------------------------------------------------------------*)
+(* Find the type of different kinds of expressions                           *)
 
-Fixpoint connect_non_passive (ct_old : module_graph_connection_trees_p.env)
-                             (ref_tgt : HiFP.href) (lst_tgt : list PProdVarOrder.t) (ft_tgt : ftype)
-                             (ref_src : HiFP.href) (lst_src : list PProdVarOrder.t) (ft_src : ftype)
-                             (ct_new : module_graph_connection_trees_p.env) : bool :=
-   (* The predicate returns true if the correct connection trees are in ct_new
-      that connect from lst_src to lst_tgt, and that the connection trees that
-      connect to lst_src are not changed.  Other connection trees are not checked.
-      The type of lst_tgt is ft_tgt, and the type of lst_src is ft_src.
-      These references are *not* required to have passive types.
+(* The functions in this part mostly rely on the tmap, the type map based on
+   the ports and statements in the module.  Note that the module graph might
+   contain different widths for implicit-width components. *)
 
-      We copy the same code two times, to allow Coq to prove that the recursion is well-founded. *)
-   match ft_tgt, ft_src with
-   | Gtyp gt_tgt, Gtyp gt_src => connect_non_passive_fgtyp ct_old ref_tgt lst_tgt gt_tgt ref_src lst_src gt_src ct_new
-   | Atyp elt_tgt n1, Atyp elt_src n2 => (n1 == n2) &&
-      let type_len := size_of_ftype elt_tgt in
-            (size lst_tgt == type_len * n1) && (size lst_src == type_len * n1)
-         &&
-            [forall n : ordinal n1,
-               connect_non_passive ct_old
-                                   (Esubindex ref_tgt n) (take type_len (drop (n * type_len) lst_tgt)) elt_tgt
-                                   (Esubindex ref_src n) (take type_len (drop (n * type_len) lst_src)) elt_src
-                                   ct_new]
-   | Btyp ff_tgt, Btyp ff_src => connect_non_passive_fields ct_old ref_tgt lst_tgt ff_tgt ref_src lst_src ff_src ct_new
-   | _, _ => false
-   end
-with connect_non_passive_fields (ct_old : module_graph_connection_trees_p.env)
-                                (ref_tgt : HiFP.href) (lst_tgt : list PProdVarOrder.t) (ft_tgt : ffield)
-                                (ref_src : HiFP.href) (lst_src : list PProdVarOrder.t) (ft_src : ffield)
-                                (ct_new : module_graph_connection_trees_p.env) : bool :=
-   (* The predicate returns true if the correct connection trees are in ct_new
-      that connect from lst_src to lst_tgt, and that the connection trees that
-      connect to lst_src are not changed.  Other connection trees are not checked.
-      The type of lst_tgt is (Btyp ft_tgt), and the type of lst_src is (Btyp ft_src).
-      These references are *not* required to have passive types.
-
-      We copy the same code two times, to allow Coq to prove that the recursion is well-founded. *)
-   match ft_tgt, ft_src with
-   | Fnil, Fnil => true
-   | Fflips v1 Nflip gtt ft, Fflips v2 Nflip gts fs => (v1 == v2) &&
-         let type_len := size_of_ftype gtt in
-               connect_non_passive ct_old (Esubfield ref_tgt v1) (take type_len lst_tgt) gtt (Esubfield ref_src v2) (take type_len lst_src) gts ct_new
-            &&
-               connect_non_passive_fields ct_old ref_tgt (drop type_len lst_tgt) ft ref_src (drop type_len lst_src) fs ct_new
-   | Fflips v1 Flipped gtt ft, Fflips v2 Flipped gts fs => (v1 == v2) &&
-         let type_len := size_of_ftype gts in
-               connect_non_passive_flipped ct_old (Esubfield ref_src v2) (take type_len lst_src) gts (Esubfield ref_tgt v1) (take type_len lst_tgt) gtt ct_new
-            &&
-               connect_non_passive_fields ct_old ref_tgt (drop type_len lst_tgt) ft ref_src (drop type_len lst_src) fs ct_new
-   | _, _ => false
-   end
-with connect_non_passive_flipped (ct_old : module_graph_connection_trees_p.env)
-                                 (ref_tgt : HiFP.href) (lst_tgt : list PProdVarOrder.t) (ft_tgt : ftype)
-                                 (ref_src : HiFP.href) (lst_src : list PProdVarOrder.t) (ft_src : ftype)
-                                 (ct_new : module_graph_connection_trees_p.env) : bool :=
-   (* The code in this predicate is the same as in connect_non_passive. *)
-   match ft_tgt, ft_src with
-   | Gtyp gt_tgt, Gtyp gt_src => connect_non_passive_fgtyp ct_old ref_tgt lst_tgt gt_tgt ref_src lst_src gt_src ct_new
-   | Atyp elt_tgt n1, Atyp elt_src n2 => (n1 == n2) &&
-      let type_len := size_of_ftype elt_tgt in
-            (size lst_tgt == type_len * n1) && (size lst_src == type_len * n1)
-         &&
-            [forall n : ordinal n1,
-               connect_non_passive_flipped ct_old
-                                           (Esubindex ref_tgt n) (take type_len (drop (n * type_len) lst_tgt)) elt_tgt
-                                           (Esubindex ref_src n) (take type_len (drop (n * type_len) lst_src)) elt_src
-                                           ct_new]
-
-   | Btyp ff_tgt, Btyp ff_src => connect_non_passive_fields_flipped ct_old ref_tgt lst_tgt ff_tgt ref_src lst_src ff_src ct_new
-   | _, _ => false
-   end
-with connect_non_passive_fields_flipped (ct_old : module_graph_connection_trees_p.env)
-                                        (ref_tgt : HiFP.href) (lst_tgt : list PProdVarOrder.t) (ft_tgt : ffield)
-                                        (ref_src : HiFP.href) (lst_src : list PProdVarOrder.t) (ft_src : ffield)
-                                        (ct_new : module_graph_connection_trees_p.env) : bool :=
-   (* The code in this predicate is the same as in connect_non_passive_fields. *)
-   match ft_tgt, ft_src with
-   | Fnil, Fnil => true
-   | Fflips v1 Nflip gtt ft, Fflips v2 Nflip gts fs => (v1 == v2) &&
-         let type_len := size_of_ftype gtt in
-               connect_non_passive_flipped ct_old (Esubfield ref_tgt v1) (take type_len lst_tgt) gtt (Esubfield ref_src v2) (take type_len lst_src) gts ct_new
-            &&
-               connect_non_passive_fields_flipped ct_old ref_tgt (drop type_len lst_tgt) ft ref_src (drop type_len lst_src) fs ct_new
-   | Fflips v1 Flipped gtt ft, Fflips v2 Flipped gts fs => (v1 == v2) &&
-         let type_len := size_of_ftype gts in
-               connect_non_passive ct_old (Esubfield ref_src v2) (take type_len lst_src) gts (Esubfield ref_tgt v1) (take type_len lst_tgt) gtt ct_new
-            &&
-               connect_non_passive_fields_flipped ct_old ref_tgt (drop type_len lst_tgt) ft ref_src (drop type_len lst_src) fs ct_new
-   | _, _ => false
-   end.
-
-Fixpoint connect_type_compatible (ft_ref : ftype) (ft_expr : ftype_explicit) : bool :=
-(* returns true iff a signal of type ft_expr can be connected to ft_ref.
-   It also ensures that the types are passive. *)
-   match ft_ref, ft_expr with
-   | Gtyp (Fuint _), exist (Gtyp (Fuint _)) _
-   | Gtyp (Fsint _), exist (Gtyp (Fsint _)) _
-   | Gtyp Fclock, exist (Gtyp Fclock) _
-   | Gtyp Fasyncreset, exist (Gtyp Fasyncreset) _ => true
-   | Gtyp (Fuint_implicit w_ref), exist (Gtyp (Fuint w_expr)) _
-   | Gtyp (Fsint_implicit w_ref), exist (Gtyp (Fsint w_expr)) _ => w_ref >= w_expr
-   | Atyp t_ref n_ref, exist (Atyp t_expr n_expr) p => connect_type_compatible t_ref (exist ftype_not_implicit_width t_expr p) && (n_ref == n_expr)
-   | Btyp ff_ref, exist (Btyp ff_expr) p => connect_type_compatible_fields ff_ref (exist ffield_not_implicit_width ff_expr p)
-   | _, _ => false
-   end
-with connect_type_compatible_fields (ff_ref : ffield) (ff_expr : ffield_explicit) : bool :=
-   match ff_ref, ff_expr with
-   | Fnil, exist Fnil _ => true
-   | Fflips v_ref Nflip t_ref ff_ref', exist (Fflips v_expr Nflip t_expr ff_expr') p =>
-          (v_ref == v_expr) && connect_type_compatible t_ref (exist ftype_not_implicit_width t_expr (proj1 p))
-                            && connect_type_compatible_fields ff_ref' (exist ffield_not_implicit_width ff_expr' (proj2 p))
-   | _, _ => false
-   end.
-
-Fixpoint list_rhs_ref_p (ref : HiFP.href) (ft : ftype) : option (seq HiFP.hfexpr) :=
-(* Finds expressions for the ground-type components of the reference ref, which is of type ft.
-   ft must be a passive type. *)
-match ft with
-| Gtyp _ => Some [:: Eref ref]
-| Atyp t n =>
-    iteri n (fun (i : nat) (ol : option (seq HiFP.hfexpr)) =>
-                 match ol, list_rhs_ref_p (Esubindex ref i) t with
-                 | Some l, Some li => Some (l ++ li)
-                 | _, _ => None
-                 end)
-          (Some [::])
-| Btyp ff => list_rhs_ref_p_fields ref ff
-end
-with list_rhs_ref_p_fields (ref : HiFP.href) (ff : ffield) : option (seq HiFP.hfexpr) :=
-match ff with
-| Fnil => Some [::]
-| Fflips v Nflip t ff' =>
-    match list_rhs_ref_p (Esubfield ref v) t, list_rhs_ref_p_fields ref ff' with
-    | Some l1, Some l2 => Some (l1 ++ l2)
-    | _, _ => None
-    end
-| Fflips _ Flipped _ _ => None
-end.
-
-Fixpoint list_rhs_expr_p (expr : HiFP.hfexpr) (ft : ftype) : option (seq HiFP.hfexpr) :=
-(* Finds ground-type components of the expression expr, which is of type ft.
-   Does not do type checking but just assumes that expr has type ft.
-   If the type is not a ground type, then the expression must be either a reference or a multiplexer. *)
-if ft is Gtyp _ then Some [:: expr]
-else match expr with
-     | Emux c e1 e2 =>
-         match list_rhs_expr_p e1 ft, list_rhs_expr_p e2 ft with
-         | Some l1, Some l2 =>
-             if size l1 == size l2
-             then Some (map (fun (e12 : HiFP.hfexpr * HiFP.hfexpr) => Emux c (fst e12) (snd e12)) (zip l1 l2))
-             else None
-         | _, _ => None
-         end
-   (*| Evalidif c e =>
-         match list_rhs_expr_p e ft with
-         | Some l =>
-             Some (map (fun (ee : HiFP.hfexpr) => Evalidif c ee) l)
-         | None => None
-         end*)
-     | Eref ref => list_rhs_ref_p ref ft
-     | _ => None
-     end.
-
-Fixpoint list_rhs_type_p (ft : ftype) : seq fgtyp :=
-(* Finds the types of ground-type components of type ft.
-   (In contrast to the older function vtype_list, this function does not convert Freset to
-   Fuint 1 or Fasyncreset.) *)
-match ft with
-| Gtyp gt => [:: gt]
-| Atyp ft' m => let elt_list := list_rhs_type_p ft' in
-                (* append m copies of elt_list to the empty list: *)
-                iter m (fun (ll : seq fgtyp) => ll ++ elt_list) [::]
-| Btyp ff => list_rhs_ffield_p ff
-end
-with list_rhs_ffield_p (ff : ffield) : seq fgtyp :=
-match ff with
-| Fnil => [::]
-| Fflips _ _ ft' ff' => (list_rhs_type_p ft') ++ (list_rhs_ffield_p ff')
-end.
-
-(* Find the type of different kinds of expressions: *)
-
-Fixpoint type_of_ffield (v : VarOrder.t) (ff : ffield) : option ftype :=
+Fixpoint type_of_ffield (v : VarOrder.T) (ff : ffield) : option ftype :=
 (* Find the type of field v in bundle type (Btyp ff). *)
 match ff with
 | Fnil => None
 | Fflips v0 _ t ff' => if v == v0 then Some t else type_of_ffield v ff'
 end.
 
-Fixpoint type_of_ref (ref : HiFP.href) (tmap : ft_pmap) : option ftype :=
-(* Find the type of reference ref, using the type information from tmap. *)
+Fixpoint type_of_ref (ref : HiFP.href) (tmap : CEP.t ftype) : option ftype :=
+(* Find the type of reference ref, using the type information from tmap.
+   Note that widths of implicit-width components may be wrong.
+
+   This function is similar to base_ref; check whether they can be made more similar. *)
 match ref with
-| Eid v => ft_find v tmap
+| Eid v => CEP.find v tmap
 | Esubindex ref' n =>
     match type_of_ref ref' tmap with
     | Some (Atyp t m) => if n < m then Some t else None
@@ -507,72 +263,6 @@ match ref with
 | Esubaccess _ _ => None
 end.
 
-Definition tmap_subset (t1 t2: ft_pmap) : Prop :=
-forall v : ProdVarOrder.T,
-   match ft_find v t1 with
-   | Some ft => ft_find v t2 = Some ft
-   | None => True
-   end.
-
-Lemma tmap_subset_refl : forall tmap : ft_pmap, tmap_subset tmap tmap.
-Proof.
-unfold tmap_subset ; intros.
-destruct (ft_find v tmap) ; done.
-Qed.
-
-Lemma tmap_subset_trans : forall t2 t1 t3 : ft_pmap, tmap_subset t1 t2 -> tmap_subset t2 t3 -> tmap_subset t1 t3.
-Proof.
-unfold tmap_subset ; intros.
-specialize H with (v := v) ; specialize H0 with (v := v).
-destruct (ft_find v t1) ; last by trivial.
-rewrite H in H0.
-exact H0.
-Qed.
-
-Lemma tmap_subset_add : forall (tmap : ft_pmap) (v : N * N) (t : ftype),
-   ft_find v tmap = None -> tmap_subset tmap (ft_add v t tmap).
-Proof.
-unfold ft_add, tmap_subset, ft_find at 3.
-intros.
-destruct (v0 == v) eqn: Hv ; rewrite Hv.
-* move /eqP : Hv => Hv ; rewrite Hv H //.
-* destruct (ft_find v0 tmap) ; by done.
-Qed.
-
-Lemma tmap_subset_add_add : forall (tmap1 tmap2 : ft_pmap) (v : N * N) (t : ftype),
-   tmap_subset tmap1 tmap2 -> tmap_subset (ft_add v t tmap1) (ft_add v t tmap2).
-Proof.
-unfold ft_add, tmap_subset, ft_find at 3 5.
-intros.
-specialize H with (v := v0).
-destruct (ft_find v0 tmap1) ; simpl.
-* rewrite H.
-  destruct (if v0 == v then Some t else Some f) eqn: H0 ; rewrite H0 ; done.
-* destruct (v0 == v) eqn: H0 ; rewrite H0 ; done.
-Qed.
-
-Lemma type_of_ref_subset : forall (ref : HiFP.href) (tmap1 tmap2 : ft_pmap),
-   tmap_subset tmap1 tmap2 ->
-   match type_of_ref ref tmap1 with
-   | Some ft => type_of_ref ref tmap2 = Some ft
-   | None => True
-   end.
-Proof.
-intros.
-induction ref ; simpl ; try trivial.
-* by apply H.
-* destruct (type_of_ref ref tmap1) ; last by trivial.
-  rewrite IHref.
-  destruct f ; first (by trivial) ; first by trivial.
-  destruct (type_of_ffield v f) ; last by trivial.
-  by reflexivity.
-* destruct (type_of_ref ref tmap1) ; last by trivial.
-  rewrite IHref.
-  destruct f ; first (by trivial) ; last by trivial.
-  destruct (n < n0) ; last by trivial.
-  by reflexivity.
-Qed.
-
 Definition fgtyp_mux (x y : fgtyp_explicit) : option fgtyp_explicit :=
 (* Find the type of a multiplexer whose two inputs have types x and y, for ground types *)
     match x, y with
@@ -585,8 +275,9 @@ Definition fgtyp_mux (x y : fgtyp_explicit) : option fgtyp_explicit :=
     end.
 
 Fixpoint ftype_mux' (x : ftype) (px : ftype_not_implicit_width x) (y : ftype) (py : ftype_not_implicit_width y) : option ftype_explicit :=
-(* Find the type of a multiplexer whose two inputs have types x and y, for ground types.
-   The function needs to take apart the ftype_explicit so Coq can guess the decreasing argument *)
+(* Find the type of a multiplexer whose two inputs have types (exist ftype_not_implicit_width x px)
+   and (exist ftype_not_implicit_width y py).
+   The function needs to take apart the ftype_explicit so Coq can guess the decreasing argument. *)
   match x, px, y, py with
   | Gtyp tx, px, Gtyp ty, py =>
        match fgtyp_mux (exist not_implicit_width tx px) (exist not_implicit_width ty py) with
@@ -618,11 +309,15 @@ with ffield_mux' (f1 : ffield) (p1 : ffield_not_implicit_width f1) (f2 : ffield)
        end.
 
 Definition ftype_mux (x : ftype_explicit) (y : ftype_explicit) : option ftype_explicit :=
-(* return the type of mux expression on ftypes *)
+(* return the type of mux expression on ftypes
+
+   Similar to mux_types in InferWidths *)
    ftype_mux' (proj1_sig x) (proj2_sig x) (proj1_sig y) (proj2_sig y).
 
-Fixpoint type_of_expr (expr : HiFP.hfexpr) (tmap: ft_pmap) : option ftype_explicit :=
-   (* Find the type of expression expr *)
+Fixpoint type_of_expr (expr : HiFP.hfexpr) (tmap: CEP.t ftype) : option ftype_explicit :=
+   (* Find the type of expression expr.
+
+   Similar to type_of_hfexpr in InferWidths *)
    match expr with
    | Econst t bs => match t with
                     | Fuint_implicit w => Some (exist ftype_not_implicit_width (Gtyp (Fuint w)) I)
@@ -772,8 +467,248 @@ Fixpoint type_of_expr (expr : HiFP.hfexpr) (tmap: ft_pmap) : option ftype_explic
    | _ => None (* Some (exist ftype_not_implicit_width (Gtyp (Fuint 0)) I) *)
    end.
 
-Lemma type_of_expr_subset : forall (expr : HiFP.hfexpr) (tmap1 tmap2 : ft_pmap),
-   tmap_subset tmap1 tmap2 ->
+
+(*---------------------------------------------------------------------------*)
+(* Find the tmap of ports and of statements                                  *)
+
+(* Tmaps store the type of every component in a module.  The type information
+   is taken from the module, but the width is corrected according to the
+   module graph. *)
+
+Definition code_vm_type_equivalent (code_type : fgtyp) (graph_type : fgtyp) : bool :=
+(* check whether types code_type and graph_type are equivalent.
+   graph_type should be allowed in a module graph (i.e. it cannot be Freset). *)
+match code_type, graph_type with
+| Fuint w1, Fuint w2
+| Fsint w1, Fsint w2 => w1 == w2
+| Fuint_implicit _, Fuint_implicit _
+| Fsint_implicit _, Fsint_implicit _
+| Fclock, Fclock
+| Freset, Fuint 1
+| Freset, Fasyncreset
+| Fasyncreset, Fasyncreset => true
+| _, _ => false
+end.
+
+Fixpoint code_type_find_vm_widths (code_t : ftype) (v : ProdVarOrder.T) (vm : module_graph_vertex_set_p.env) : option (ftype * N) :=
+(* find the widths of types used in vm for a component that was declared with type code_t in the code.
+   The module graph vertices (v, n), (v, n+1), (v, n+2), ... contain the relevant ground-type subcomponents.
+   That means, the module graph vertices should contain ground-type elements as given by code_vm_type_equivalent.
+   The result is a pair:
+   - the type with widths adapted
+   - the new index for n (where the next subcomponent would be found after handling code_t)
+     (i.e. n + size_of_ftype code_t)
+   If there is some error, the result is None instead.
+   We allow non-passive types.
+   Note that in most cases, the type of the output of the component is used,
+   but for OutPorts we use the type of the input (because an out-port has no output connector). *)
+match code_t with
+| Gtyp oldgt =>
+    match module_graph_vertex_set_p.find v vm with
+    | Some (OutPort newgt)
+    | Some (InPort newgt)
+    | Some (Register newgt)
+    | Some (RegisterReset newgt _)
+    | Some (Wire newgt)
+    | Some (Node newgt) =>
+        if code_vm_type_equivalent oldgt newgt
+        then Some (Gtyp newgt, N.of_nat (snd v + 1))
+        else None
+    | None => None
+    end
+| Atyp code_t' m =>
+    (* check the first copy, and then verify that the next m-1 copies have exactly the same types *)
+    match code_type_find_vm_widths code_t' v vm with
+    | Some (graph_t', new_n) =>
+        (* Now check that there are another m-1 copies that are identical *)
+        let elsize := N.sub new_n (snd v) in
+        if [forall i : ordinal ((m-1) * elsize),
+               module_graph_vertex_set_p.find (fst v, N.add (snd v) (N.of_nat i)) vm ==
+               module_graph_vertex_set_p.find (fst v, N.add new_n   (N.of_nat i)) vm   ]
+        then Some (Atyp graph_t' m, N.add (snd v) (N.mul (N.of_nat m) elsize))
+        else None
+    | None => None
+    end
+| Btyp code_ff => code_ffield_find_vm_widths code_ff v vm
+end
+with code_ffield_find_vm_widths (code_ff : ffield) (v : ProdVarOrder.T) (vm : module_graph_vertex_set_p.env) : option (ftype * N) :=
+match code_ff with
+| Fnil => Some (Btyp Fnil, snd v)
+| Fflips f flp code_t code_ff' =>
+    match code_type_find_vm_widths code_t v vm with
+    | Some (graph_t, n') =>
+        match code_ffield_find_vm_widths code_ff' (fst v, n') vm with
+        | Some (Btyp graph_ff, n'') =>
+            Some (Btyp (Fflips f flp graph_t graph_ff), n'')
+        | _ => None
+        end
+    | None => None
+    end
+end.
+
+Fixpoint ports_tmap (pp : seq HiFP.hfport) (vm : module_graph_vertex_set_p.env) : option (CEP.t ftype) :=
+(* creates a tmap that contains exactly the types of the ports in pp. *)
+match pp with
+| [::] => Some (CEP.empty ftype)
+| Finput v t :: pp'
+| Foutput v t :: pp' =>
+    match code_type_find_vm_widths t v vm, ports_tmap pp' vm with
+    | Some (newt, _), Some tmap' => Some (CEP.add v newt tmap')
+    | _, _ => None
+    end
+end.
+
+Fixpoint stmts_tmap (tmap_scope : CEP.t ftype * CEP.t ftype) (ss : HiFP.hfstmt_seq) (vm : module_graph_vertex_set_p.env) : option (CEP.t ftype * CEP.t ftype) :=
+(* extends tmap_scope with the types of the defined components in ss.
+   The first part of tmap_scope contains all defined components
+   (used to check for name clashes, and will also be used later in Sem_frag_stmt);
+   the second part contains only the components in the current scope
+   (used to check whether a component defined within a Swhen statement
+   is illegally used outside it).
+   Produces None if some component is defined more than once,
+   if a component is accessed before it is defined,
+   or if it is accessed out of scope.
+
+   Problem: does not check the directionality of the component
+   (e.g. a node can only be read, an output port can only be written).
+   Should we replace the tmap with a component environment? *)
+match ss with
+| Qnil => Some tmap_scope
+| Qcons s ss' =>
+    match stmt_tmap tmap_scope s vm with
+    | Some tmap_scope' => stmts_tmap tmap_scope' ss' vm
+    | None => None
+    end
+end
+with stmt_tmap (tmap_scope : CEP.t ftype * CEP.t ftype) (s : HiFP.hfstmt) (vm : module_graph_vertex_set_p.env) : option (CEP.t ftype * CEP.t ftype) :=
+(* extends tmap_scope with the type of the component defined in s.
+   Produces None if s contains a definition of a component that is already in tmap. *)
+match s with
+| Sskip => Some tmap_scope
+| Sfcnct ref expr =>
+    match type_of_ref ref (snd tmap_scope), type_of_expr expr (snd tmap_scope) with
+    | Some _, Some _ => Some tmap_scope
+    | _, _ => None (* something undefined or out-of-scope is accessed *)
+    end
+| Sinvalid ref =>
+    match type_of_ref ref (snd tmap_scope) with
+    | Some _ => Some tmap_scope
+    | None => None (* ref is undefined or out of scope *)
+    end
+| Swire v t =>
+    match CEP.find v (fst tmap_scope), code_type_find_vm_widths t v vm with
+    | None, Some (newt, _) =>
+        Some (CEP.add v newt (fst tmap_scope), CEP.add v newt (snd tmap_scope))
+    | _, _ => None (* identifier v is used multiple times, or the module graph does not fit *)
+    end
+| Sreg v reg =>
+    match CEP.find v (fst tmap_scope), code_type_find_vm_widths (type reg) v vm with
+    | None, Some (newt, _) =>
+        if reset reg is Rst rst_sig rst_val
+        then match type_of_expr rst_sig (snd tmap_scope), type_of_expr rst_val (snd tmap_scope) with
+             | Some _, Some _ => Some (CEP.add v newt (fst tmap_scope), CEP.add v newt (snd tmap_scope))
+             | _, _ => None (* something undefined or out-of-scope is accessed *)
+             end
+        else Some (CEP.add v newt (fst tmap_scope), CEP.add v newt (snd tmap_scope))
+    | _, _ => None (* identifier v is used multiple times, or the module graph does not fit *)
+    end
+| Snode v expr =>
+    match CEP.find v (fst tmap_scope), type_of_expr expr (snd tmap_scope) with
+    | None, Some (exist newt _) =>
+        Some (CEP.add v newt (fst tmap_scope), CEP.add v newt (snd tmap_scope))
+    | _, _ => None (* something undefined or out-of-scope is accessed, or identifier v is used multiple times *)
+    end
+| Smem _ _ => None
+| Sinst _ _ => None
+| Swhen cond ss_true ss_false =>
+    match type_of_expr cond (snd tmap_scope), stmts_tmap tmap_scope ss_true vm with
+    | Some _, Some (tmap_true, _) =>
+        if stmts_tmap (tmap_true, snd tmap_scope) ss_false vm is Some (tmap_false, _)
+        then Some (tmap_false, snd tmap_scope)
+        else None (* there is an error in ss_false *)
+    | _, _ => None (* cond accesses something undefined or out-of-scope, or there is an error in ss_true *)
+    end
+end.
+
+
+(*---------------------------------------------------------------------------*)
+(* Submaps                                                                   *)
+
+Definition submap {T : Type} (t1 t2: CEP.t T) : Prop :=
+forall v : ProdVarOrder.T,
+   match CEP.find v t1 with
+   | Some ft => CEP.find v t2 = Some ft
+   | None => True
+   end.
+
+Lemma submap_refl : forall tmap : CEP.t ftype, submap tmap tmap.
+Proof.
+unfold submap ; intros.
+destruct (CEP.find v tmap) ; done.
+Qed.
+
+Lemma submap_trans : forall t2 t1 t3 : CEP.t ftype, submap t1 t2 -> submap t2 t3 -> submap t1 t3.
+Proof.
+unfold submap ; intros.
+specialize H with (v := v) ; specialize H0 with (v := v).
+destruct (CEP.find v t1) ; last by trivial.
+rewrite H in H0.
+exact H0.
+Qed.
+
+Lemma submap_add : forall (tmap : CEP.t ftype) (v : N * N) (t : ftype),
+   CEP.find v tmap = None -> submap tmap (CEP.add v t tmap).
+Proof.
+unfold submap.
+intros.
+destruct (v0 == v) eqn: Hv.
+* rewrite CEP.Lemmas.find_add_eq ; last by rewrite /HiFirrtl.PVM.SE.eq Hv //.
+  move /eqP : Hv => Hv ; rewrite Hv H //.
+* rewrite CEP.Lemmas.find_add_neq ; last by rewrite /HiFirrtl.PVM.SE.eq Hv //.
+  destruct (CEP.find v0 tmap) ; done.
+Qed.
+
+Lemma submap_add_add : forall (tmap1 tmap2 : CEP.t ftype) (v : N * N) (t : ftype),
+   submap tmap1 tmap2 -> submap (CEP.add v t tmap1) (CEP.add v t tmap2).
+Proof.
+unfold submap.
+intros.
+destruct (v0 == v) eqn: Hv.
+* rewrite CEP.Lemmas.find_add_eq ; last by rewrite /HiFirrtl.PVM.SE.eq Hv //.
+  rewrite CEP.Lemmas.find_add_eq ; last by rewrite /HiFirrtl.PVM.SE.eq Hv //.
+  reflexivity.
+* rewrite CEP.Lemmas.find_add_neq ; last by rewrite /HiFirrtl.PVM.SE.eq Hv //.
+  rewrite CEP.Lemmas.find_add_neq ; last by rewrite /HiFirrtl.PVM.SE.eq Hv //.
+  apply H.
+Qed.
+
+(*---------------------------------------------------------------------------*)
+(* Properties of type_of_ref and of type_of_expr                             *)
+
+Lemma type_of_ref_submap : forall (ref : HiFP.href) (tmap1 tmap2 : CEP.t ftype),
+   submap tmap1 tmap2 ->
+   match type_of_ref ref tmap1 with
+   | Some ft => type_of_ref ref tmap2 = Some ft
+   | None => True
+   end.
+Proof.
+intros.
+induction ref ; simpl ; try trivial.
+* by apply H.
+* destruct (type_of_ref ref tmap1) ; last by trivial.
+  rewrite IHref.
+  destruct f ; first (by trivial) ; first by trivial.
+  destruct (type_of_ffield v f) ; last by trivial.
+  by reflexivity.
+* destruct (type_of_ref ref tmap1) ; last by trivial.
+  rewrite IHref.
+  destruct f ; first (by trivial) ; last by trivial.
+  destruct (n < n0) ; last by trivial.
+  by reflexivity.
+Qed.
+
+Lemma type_of_expr_submap : forall (expr : HiFP.hfexpr) (tmap1 tmap2 : CEP.t ftype),
+   submap tmap1 tmap2 ->
    match type_of_expr expr tmap1 with
    | Some ft => type_of_expr expr tmap2 = Some ft
    | None => True
@@ -835,80 +770,642 @@ induction expr ; simpl ; try trivial.
   destruct n ; first by trivial.
   destruct n ; last by trivial.
   by reflexivity.
-* apply type_of_ref_subset with (ref := h) in H.
+* apply type_of_ref_submap with (ref := h) in H.
   destruct (type_of_ref h tmap1) ; try by trivial.
   rewrite H.
   by reflexivity.
 Qed.
 
-Definition vtype_equivalent (code_type : fgtyp) (graph_type : fgtyp) : bool :=
-(* check whether types code_type and graph_type are equivalent.
-   graph_type should be allowed in a module graph (i.e. it cannot be Freset). *)
-match code_type, graph_type with
-| Fuint w1, Fuint w2
-| Fsint w1, Fsint w2 => w1 == w2
-| Fuint_implicit _, Fuint_implicit _
-| Fsint_implicit _, Fsint_implicit _
-| Fclock, Fclock
-| Freset, Fuint 1
-| Freset, Fuint_implicit 1 (* should this really be included? It might break the property that widening of implicit types is always ok. *)
-| Freset, Fasyncreset
-| Fasyncreset, Fasyncreset => true
-| _, _ => false
+Lemma stmts_submap:
+   forall (vm : module_graph_vertex_set_p.env) (ss : HiFP.hfstmt_seq) (tmap scope : CEP.t ftype),
+      submap scope tmap ->
+         match stmts_tmap (tmap, scope) ss vm with
+         | Some (tmap', scope') => submap scope' tmap' /\ submap tmap tmap' /\ submap scope scope'
+         | None => True
+         end
+with stmt_submap :
+   forall (vm : module_graph_vertex_set_p.env) (s : HiFP.hfstmt) (tmap scope : CEP.t ftype),
+      submap scope tmap ->
+         match stmt_tmap (tmap, scope) s vm with
+         | Some (tmap', scope') => submap scope' tmap' /\ submap tmap tmap' /\ submap scope scope'
+         | None => True
+         end.
+Proof.
+* clear stmts_submap.
+  induction ss.
+  + unfold stmts_tmap.
+    intros ; split ; first by exact H.
+    by split ; apply submap_refl.
+  + intros.
+    simpl stmts_tmap.
+    specialize stmt_submap with (vm := vm) (s := h) (tmap := tmap) (scope := scope).
+    destruct (stmt_tmap (tmap, scope) h vm) as [[tmap' scope']|] ; last by trivial.
+    specialize IHss with (tmap := tmap') (scope := scope').
+    destruct (stmts_tmap (tmap', scope') ss vm) as [[tmap'' scope'']|] ; last by trivial.
+    split.
+    - apply IHss, stmt_submap, H.
+    split.
+    - apply (submap_trans tmap') ; first by apply stmt_submap.
+      by apply IHss, stmt_submap, H.
+    - apply (submap_trans scope') ; first by apply stmt_submap.
+      by apply IHss, stmt_submap, H.
+* clear stmt_submap.
+  destruct s ; simpl ; intros ; try trivial.
+  + (* Sskip *) split ; first by exact H.
+    by split ; apply submap_refl.
+  + (* Swire *)
+    destruct (CEP.find s tmap) eqn: Hfind ; first by trivial.
+    destruct (code_type_find_vm_widths f s vm) as [[newt _]|] ; last by trivial.
+    split.
+    - by apply submap_add_add, H.
+    split.
+    - by apply submap_add, Hfind.
+    - apply submap_add.
+      unfold submap in H ; specialize H with (v := s).
+      destruct (CEP.find s scope) ; last by trivial.
+      by rewrite -H -Hfind //.
+  + (* Sreg *)
+    destruct (CEP.find s tmap) eqn: Hfind ; first by trivial.
+    destruct (code_type_find_vm_widths (type h) s vm) as [[newt _]|] ; last by trivial.
+    destruct (reset h).
+    - split.
+      * by apply submap_add_add, H.
+      split.
+      * by apply submap_add, Hfind.
+      * apply submap_add.
+        unfold submap in H ; specialize H with (v := s).
+        destruct (CEP.find s scope) ; last by trivial.
+        by rewrite -H -Hfind //.
+    - destruct (type_of_expr h0 scope) ; last by trivial.
+      destruct (type_of_expr h1 scope) ; last by trivial.
+      split.
+      * by apply submap_add_add, H.
+      split.
+      * by apply submap_add, Hfind.
+      * apply submap_add.
+        unfold submap in H ; specialize H with (v := s).
+        destruct (CEP.find s scope) ; last by trivial.
+        by rewrite -H -Hfind //.
+  + (* Snode *)
+    destruct (CEP.find s tmap) eqn: Hfind ; first by trivial.
+    destruct (type_of_expr h scope) as [[newt _]|] ; last by trivial.
+    split.
+    - by apply submap_add_add, H.
+    split.
+    - by apply submap_add, Hfind.
+    - apply submap_add.
+      unfold submap in H ; specialize H with (v := s).
+      destruct (CEP.find s scope) ; last by trivial.
+      by rewrite -H -Hfind //.
+  + (* Sfcnct *)
+    destruct (type_of_ref h scope) ; last by trivial.
+    destruct (type_of_expr h0 scope) ; last by trivial.
+    split.
+    - by exact H.
+    - split ; by apply submap_refl.
+  + (* Sinvalid *)
+    destruct (type_of_ref h scope) ; last by trivial.
+    split.
+    - by exact H.
+    - split ; by apply submap_refl.
+  + (* Swhen *)
+    rename h0 into ss_true ; rename h1 into ss_false.
+    destruct (type_of_expr h scope) ; last by trivial.
+    generalize (stmts_submap vm ss_true tmap scope H) ; intro.
+    destruct (stmts_tmap (tmap, scope) ss_true vm) as [[tmap_true scope_true]|] ; last by trivial.
+    generalize (stmts_submap vm ss_false tmap_true scope (submap_trans tmap _ _ H (proj1 (proj2 H0)))) ; intro.
+    destruct (stmts_tmap (tmap_true, scope) ss_false vm) as [[tmap_false scope_false]|] ; last by trivial.
+    split.
+    - apply (submap_trans tmap) ; first by apply H.
+      apply (submap_trans tmap_true) ; first by apply H0.
+      apply H1.
+    split.
+    - apply (submap_trans tmap_true) ; first by apply H0.
+      apply H1.
+    - apply submap_refl.
+Qed.
+
+Lemma stmts_tmap_cat :
+   forall (vm : module_graph_vertex_set_p.env) (ss1 ss2 : HiFP.hfstmt_seq) (tmap_scope : CEP.t ftype * CEP.t ftype),
+      stmts_tmap tmap_scope (Qcat ss1 ss2) vm =
+      match stmts_tmap tmap_scope ss1 vm with
+      | Some tmap_scope' => stmts_tmap tmap_scope' ss2 vm
+      | None => None
+      end.
+Proof.
+induction ss1.
+* simpl Qcat ; simpl stmts_tmap ; simpl.
+  by intro ; reflexivity.
+* simpl Qcat ; simpl stmts_tmap.
+  intros.
+  destruct (stmt_tmap tmap_scope h vm) ; last by reflexivity.
+  by apply IHss1.
+Qed.
+
+
+(*---------------------------------------------------------------------------*)
+(* component defining statements and their properties                        *)
+
+Fixpoint component_stmts_of (ss : HiFP.hfstmt_seq) : HiFP.hfstmt_seq :=
+(* extracts from ss the statements that define components *)
+match ss with
+| Qnil => ss
+| Qcons s ss' => Qcat (component_stmt_of s) (component_stmts_of ss')
+end
+with component_stmt_of (s : HiFP.hfstmt) : HiFP.hfstmt_seq :=
+match s with
+| Sskip
+| Sfcnct _ _
+| Sinvalid _ => Qnil ProdVarOrder.T
+| Swire _ _
+| Sreg _ _
+| Snode _ _
+| Smem _ _
+| Sinst _ _ => Qcons s (Qnil ProdVarOrder.T)
+| Swhen _ ss_true ss_false => Qcat (component_stmts_of ss_true) (component_stmts_of ss_false)
 end.
 
-Fixpoint vtype_find_widths (code_t : ftype) (v n : N) (vm : module_graph_vertex_set_p.env) : option (ftype * N) :=
-(* find the widths of types used in vm for a component that was declared with type code_t in the code.
-   That means, the module graph vertices should contain ground-type elements as given by vtype_equivalent.
-   The result is a pair:
-   - the type with widths adapted
-   - the new index for n (where the next subcomponent would be found after handling code_t)
-   If there is some error, the result is None instead.
-   We allow non-passive types.
-   Note that in most cases, the type of the output of the component is used,
-   but for OutPorts we use the type of the input (because an out-port has no output connector). *)
-match code_t with
-| Gtyp oldgt =>
-    match module_graph_vertex_set_p.find (v, n) vm with
-    | Some (OutPort newgt)
-    | Some (InPort newgt)
-    | Some (Register newgt)
-    | Some (RegisterReset newgt _)
-    | Some (Wire newgt)
-    | Some (Node newgt) =>
-        if vtype_equivalent oldgt newgt
-        then Some (Gtyp newgt, N.of_nat (n + 1))
-        else None
-    | None => None
-    end
-| Atyp code_t' m =>
-    (* check the first copy, and then verify that the next m-1 copies have exactly the same types *)
-    match vtype_find_widths code_t' v n vm with
-    | Some (graph_t', new_n) =>
-        (* Now check that there are another m-1 copies that are identical *)
-        let t'_size := new_n - n in
-        if [forall i : ordinal ((m-1) * t'_size),
-               module_graph_vertex_set_p.find (v, N.of_nat (    n + i * t'_size)) vm ==
-               module_graph_vertex_set_p.find (v, N.of_nat (new_n + i * t'_size)) vm   ]
-        then Some (Atyp graph_t' m, N.of_nat (n + m * t'_size))
-        else None
-    | None => None
-    end
-| Btyp code_ff => vfields_find_widths code_ff v n vm
-end
-with vfields_find_widths (code_ff : ffield) (v n : N) (vm : module_graph_vertex_set_p.env) : option (ftype * N) :=
-match code_ff with
-| Fnil => Some (Btyp Fnil, n)
-| Fflips f flp code_t code_ff' =>
-    match vtype_find_widths code_t v n vm with
-    | Some (graph_t, n') =>
-        match vfields_find_widths code_ff' v n' vm with
-        | Some (Btyp graph_ff, n'') =>
-            Some (Btyp (Fflips f flp graph_t graph_ff), n'')
-        | _ => None
+Definition eq_submap (ts1 ts2 : CEP.t ftype * CEP.t ftype) : Prop :=
+fst ts1 = fst ts2 /\ submap (snd ts1) (snd ts2).
+
+Lemma stmts_tmap_components :
+   forall (vm : module_graph_vertex_set_p.env) (ss : HiFP.hfstmt_seq) (tmap_scope1 tmap_scope2 : CEP.t ftype * CEP.t ftype),
+      submap (snd tmap_scope1) (fst tmap_scope1) ->
+      submap (snd tmap_scope2) (fst tmap_scope2) ->
+      eq_submap tmap_scope1 tmap_scope2 ->
+         match stmts_tmap tmap_scope1 ss vm, stmts_tmap tmap_scope2 (component_stmts_of ss) vm with
+         | Some result1, Some result2 =>
+              eq_submap result1 result2
+         | Some _, None => False
+         | _, _ => True
+         end
+with stmt_tmap_components :
+   forall (vm : module_graph_vertex_set_p.env) (s : HiFP.hfstmt) (tmap_scope1 tmap_scope2 : CEP.t ftype * CEP.t ftype),
+      submap (snd tmap_scope1) (fst tmap_scope1) ->
+      submap (snd tmap_scope2) (fst tmap_scope2) ->
+      eq_submap tmap_scope1 tmap_scope2 ->
+         match stmt_tmap tmap_scope1 s vm, stmts_tmap tmap_scope2 (component_stmt_of s) vm with
+         | Some result1, Some result2 =>
+              eq_submap result1 result2
+         | Some _, None => False
+         | _, _ => True
+         end.
+Proof.
+* clear stmts_tmap_components.
+  induction ss.
+  + unfold component_stmts_of, stmts_tmap ; done.
+  + intros.
+    simpl stmts_tmap.
+    rewrite stmts_tmap_cat.
+    specialize stmt_tmap_components with (vm := vm) (s := h) (tmap_scope1 := tmap_scope1) (tmap_scope2 := tmap_scope2).
+    generalize (stmt_submap vm h (fst tmap_scope1) (snd tmap_scope1) H) ;
+          intro ; rewrite -surjective_pairing in H2.
+    destruct (stmt_tmap tmap_scope1 h vm) as [tmap_scope1'|] ;
+          first rewrite (surjective_pairing tmap_scope1') in H2 ;
+          last by trivial.
+    generalize (stmts_submap vm (component_stmt_of h) (fst tmap_scope2) (snd tmap_scope2) H0) ;
+          intro ; rewrite -surjective_pairing in H3.
+    destruct (stmts_tmap tmap_scope2 (component_stmt_of h) vm) as [tmap_scope2'|] ;
+          first rewrite (surjective_pairing tmap_scope2') in H3.
+    - apply IHss, stmt_tmap_components ; try assumption.
+      * by apply (proj1 H2).
+      * by apply (proj1 H3).
+    - specialize IHss with (tmap_scope1 := tmap_scope1').
+      destruct (stmts_tmap tmap_scope1' ss vm) as [tmap_scope1''|] ; last by trivial.
+      apply stmt_tmap_components ; by assumption.
+* clear stmt_tmap_components.
+  intros.
+  destruct s ; simpl ; (try (by done)) ;
+        unfold eq_submap, submap in H1 ; destruct H1 ; try rewrite -H1.
+  + (* Swire *)
+    destruct (CEP.find s (fst tmap_scope1)) ; first by trivial.
+    destruct (code_type_find_vm_widths f s vm) as [[newt _]|] ; last by trivial.
+    unfold eq_submap ; split ; first by reflexivity.
+    simpl snd.
+    intro.
+    destruct (v == s) eqn: Hvs.
+    - rewrite CEP.Lemmas.find_add_eq ; last by rewrite /HiFirrtl.PVM.SE.eq Hvs //.
+      rewrite CEP.Lemmas.find_add_eq ; last by rewrite /HiFirrtl.PVM.SE.eq Hvs //.
+      by reflexivity.
+    - rewrite CEP.Lemmas.find_add_neq ; last by rewrite /HiFirrtl.PVM.SE.eq Hvs //.
+      rewrite CEP.Lemmas.find_add_neq ; last by rewrite /HiFirrtl.PVM.SE.eq Hvs //.
+      by apply H2.
+  + (* Sreg *)
+    destruct (CEP.find s (fst tmap_scope1)) ; first by trivial.
+    destruct (code_type_find_vm_widths (type h) s vm) as [[newt _]|] ; last by trivial.
+    destruct (reset h).
+    - unfold eq_submap ; split ; first by reflexivity.
+      simpl snd.
+      intro.
+      destruct (v == s) eqn: Hvs.
+      * rewrite CEP.Lemmas.find_add_eq ; last by rewrite /HiFirrtl.PVM.SE.eq Hvs //.
+        rewrite CEP.Lemmas.find_add_eq ; last by rewrite /HiFirrtl.PVM.SE.eq Hvs //.
+        by reflexivity.
+      * rewrite CEP.Lemmas.find_add_neq ; last by rewrite /HiFirrtl.PVM.SE.eq Hvs //.
+        rewrite CEP.Lemmas.find_add_neq ; last by rewrite /HiFirrtl.PVM.SE.eq Hvs //.
+        by apply H2.
+    - destruct (type_of_expr h0 (snd tmap_scope1)) eqn: Hte0 ; last by trivial.
+      assert (type_of_expr h0 (snd tmap_scope2) = Some f).
+            generalize (type_of_expr_submap h0 (snd tmap_scope1) (snd tmap_scope2)) ; intro.
+            rewrite Hte0 in H3.
+            apply H3.
+            by exact H2.
+      rewrite H3.
+      destruct (type_of_expr h1 (snd tmap_scope1)) eqn: Hte1 ; last by trivial.
+      assert (type_of_expr h1 (snd tmap_scope2) = Some f0).
+            generalize (type_of_expr_submap h1 (snd tmap_scope1) (snd tmap_scope2)) ; intro.
+            rewrite Hte1 in H4.
+            apply H4.
+            by exact H2.
+      rewrite H4.
+      unfold eq_submap ; split ; first by reflexivity.
+      simpl snd.
+      intro.
+      destruct (v == s) eqn: Hvs.
+      * rewrite CEP.Lemmas.find_add_eq ; last by rewrite /HiFirrtl.PVM.SE.eq Hvs //.
+        rewrite CEP.Lemmas.find_add_eq ; last by rewrite /HiFirrtl.PVM.SE.eq Hvs //.
+        by reflexivity.
+      * rewrite CEP.Lemmas.find_add_neq ; last by rewrite /HiFirrtl.PVM.SE.eq Hvs //.
+        rewrite CEP.Lemmas.find_add_neq ; last by rewrite /HiFirrtl.PVM.SE.eq Hvs //.
+        by apply H2.
+  + (* Snode *)
+    destruct (CEP.find s (fst tmap_scope1)) ; first by trivial.
+    destruct (type_of_expr h (snd tmap_scope1)) as [[newt p]|] eqn: Hte ; last by trivial.
+    assert (type_of_expr h (snd tmap_scope2) = Some (exist ftype_not_implicit_width newt p)).
+          generalize (type_of_expr_submap h (snd tmap_scope1) (snd tmap_scope2)) ; intro.
+          rewrite Hte in H3.
+          apply H3.
+          by exact H2.
+    rewrite H3.
+    unfold eq_submap ; split ; first by reflexivity.
+    simpl snd.
+    intro.
+    destruct (v == s) eqn: Hvs.
+    - rewrite CEP.Lemmas.find_add_eq ; last by rewrite /HiFirrtl.PVM.SE.eq Hvs //.
+      rewrite CEP.Lemmas.find_add_eq ; last by rewrite /HiFirrtl.PVM.SE.eq Hvs //.
+      by reflexivity.
+    - rewrite CEP.Lemmas.find_add_neq ; last by rewrite /HiFirrtl.PVM.SE.eq Hvs //.
+      rewrite CEP.Lemmas.find_add_neq ; last by rewrite /HiFirrtl.PVM.SE.eq Hvs //.
+      by apply H2.
+  + (* Sfcnct *)
+    destruct (type_of_ref h (snd tmap_scope1)) ; last by trivial.
+    destruct (type_of_expr h0 (snd tmap_scope1)) ; last by trivial.
+    unfold eq_submap ; split ; first by exact H1.
+    by exact H2.
+  + (* Sinvalid *)
+    destruct (type_of_ref h (snd tmap_scope1)) ; last by trivial.
+    unfold eq_submap ; split ; first by exact H1.
+    by exact H2.
+  + (* Swhen *)
+    rename h0 into ss_true ; rename h1 into ss_false.
+    destruct (type_of_expr h (snd tmap_scope1)) ; last by trivial.
+    rewrite stmts_tmap_cat.
+    generalize (stmts_tmap_components vm ss_true tmap_scope1 tmap_scope2 H H0) ; intro.
+    generalize (stmts_submap vm ss_true (fst tmap_scope1) (snd tmap_scope1) H) ;
+          intro ; rewrite -surjective_pairing in H4.
+    destruct (stmts_tmap tmap_scope1 ss_true vm) as [[tmap_true tmap_scope_true]|] eqn: Hss_true ; last by trivial.
+    generalize (stmts_submap vm (component_stmts_of ss_true) (fst tmap_scope2) (snd tmap_scope2) H0) ;
+          intro ; rewrite -surjective_pairing in H5.
+    destruct (stmts_tmap tmap_scope2 (component_stmts_of ss_true) vm) as [[tmap_true' tmap_scope_true']|] eqn: Hss_true' ;
+          last by contradict H3 ; unfold eq_submap ; split ;
+                  first (by exact H1) ; exact H2.
+    assert (submap (snd tmap_scope1) tmap_true).
+          apply (submap_trans (fst tmap_scope1)) ; first (by exact H) ;
+          apply H4.
+    assert (eq_submap (tmap_true, snd tmap_scope1) (tmap_true', tmap_scope_true')).
+          split.
+          - simpl fst ; apply H3 ; exact (conj H1 H2).
+          - simpl snd ; apply (submap_trans (snd tmap_scope2)) ; first by exact H2.
+            by apply H5.
+    generalize (stmts_tmap_components vm ss_false (tmap_true, snd tmap_scope1) (tmap_true', tmap_scope_true') H6 (proj1 H5) H7) ; intro.
+    generalize (stmts_submap vm ss_false tmap_true (snd tmap_scope1) H6) ;
+          intro.
+    destruct (stmts_tmap (tmap_true, snd tmap_scope1) ss_false vm) as [[tmap_false tmap_scope_false]|] eqn: Hss_false ; last by trivial.
+    destruct (stmts_tmap (tmap_true', tmap_scope_true') (component_stmts_of ss_false) vm) as [[tmap_false' tmap_scope_false']|] eqn: Hss_false' ;
+          last by trivial.
+    split.
+    - simpl fst ; apply H8.
+    - simpl snd.
+      apply (submap_trans tmap_scope_false) ; first by apply H9.
+      apply H8.
+Qed.
+
+
+
+
+(*****************************************************************************)
+(*                                                                           *)
+(*                             S E M A N T I C S                             *)
+(*                                                                           *)
+(*****************************************************************************)
+
+
+(*---------------------------------------------------------------------------*)
+(* Construct lists of input connectors and expressions (for connecting)      *)
+
+Fixpoint select_field (f : VarOrder.t) (l : seq PProdVarOrder.t) (ff : ffield) : option (seq PProdVarOrder.t * ftype) :=
+(* select field f from the list of input connectors l, which corresponds to type ff.
+   ff does not need to be passive, but its direction is ignored.
+   Return the corresponding output connectors, and also return the type of the field f. *)
+match ff with
+| Fflips v _ ft ff' =>
+    let elsize := size_of_ftype ft in
+    if size l < elsize then None
+    else if f == v then Some (take elsize l, ft)
+         else select_field f (drop elsize l) ff'
+| _ => None
+end.
+
+Fixpoint list_lhs_ref_p (ref : HiFP.href) (tmap : CEP.t ftype) : option (seq PProdVarOrder.t * ftype) :=
+(* find which input connectors of ground-type identifiers correspond to reference ref.
+   ground-type identifiers are vertices in the module graph (identified by a pair of N);
+   input connectors are always the triple (vertex identifier, N0).
+   Also find the type of reference ref. *)
+match ref with
+| Eid v =>
+    (* Construct a list of identifiers and find the type of v *)
+    match CEP.find v tmap with
+    | Some t =>
+        match t, snd v with
+        | Gtyp _, _
+        | _, N0 =>
+            Some (mkseq (fun i => (fst v, N.add (snd v) (N.of_nat i), N0)) (size_of_ftype t), t)
+        | _, _ => None
         end
     | None => None
     end
+| Esubfield ref' f =>
+    match list_lhs_ref_p ref' tmap with
+    | Some (l, Btyp ff) =>
+        (* Select from list l the relevant part for field f.
+           Determine which part this is based on t *)
+        select_field f l ff
+    | _ => None
+    end
+| Esubindex ref' n =>
+    match list_lhs_ref_p ref' tmap with
+    | Some (l, Atyp t m) =>
+        (* Select from list l the relevant part for array element n.
+           Determine which part this is based on t *)
+        let elsize := size_of_ftype t in
+        if (n < m) && (size l == m * elsize)
+        then Some (take elsize (drop (n * elsize) l), t)
+        else None
+    | _ => None
+    end
+| Esubaccess _ _ => None
+end.
+
+Fixpoint list_rhs_ref_p (ref : HiFP.href) (ft : ftype) : option (seq HiFP.hfexpr) :=
+(* Finds expressions for the ground-type components of the reference ref, which is of type ft.
+   ft must be a passive type. *)
+match ft with
+| Gtyp _ => Some [:: Eref ref]
+| Atyp t n =>
+    iteri n (fun (i : nat) (ol : option (seq HiFP.hfexpr)) =>
+                 match ol, list_rhs_ref_p (Esubindex ref i) t with
+                 | Some l, Some li => Some (l ++ li)
+                 | _, _ => None
+                 end)
+          (Some [::])
+| Btyp ff => list_rhs_ref_p_fields ref ff
+end
+with list_rhs_ref_p_fields (ref : HiFP.href) (ff : ffield) : option (seq HiFP.hfexpr) :=
+match ff with
+| Fnil => Some [::]
+| Fflips v Nflip t ff' =>
+    match list_rhs_ref_p (Esubfield ref v) t, list_rhs_ref_p_fields ref ff' with
+    | Some l1, Some l2 => Some (l1 ++ l2)
+    | _, _ => None
+    end
+| Fflips _ Flipped _ _ => None
+end.
+
+Fixpoint list_rhs_expr_p (expr : HiFP.hfexpr) (ft : ftype) : option (seq HiFP.hfexpr) :=
+(* Finds ground-type components of the expression expr, which is of type ft.
+   Does not do type checking but just assumes that expr has type ft.
+   If the type is not a ground type, then the expression must be either a reference or a multiplexer. *)
+if ft is Gtyp _ then Some [:: expr]
+else match expr with
+     | Emux c e1 e2 =>
+         match list_rhs_expr_p e1 ft, list_rhs_expr_p e2 ft with
+         | Some l1, Some l2 =>
+             if size l1 == size l2
+             then Some (map (fun (e12 : HiFP.hfexpr * HiFP.hfexpr) => Emux c (fst e12) (snd e12)) (zip l1 l2))
+             else None
+         | _, _ => None
+         end
+   (*| Evalidif c e =>
+         match list_rhs_expr_p e ft with
+         | Some l =>
+             Some (map (fun (ee : HiFP.hfexpr) => Evalidif c ee) l)
+         | None => None
+         end*)
+     | Eref ref => list_rhs_ref_p ref ft
+     | _ => None
+     end.
+
+Fixpoint list_rhs_type_p (ft : ftype) : seq fgtyp :=
+(* Finds the types of ground-type components of type ft.
+   (In contrast to the older function vtype_list, this function does not convert Freset to
+   Fuint 1 or Fasyncreset.)
+
+   Probably the same as ft_find_sub. *)
+match ft with
+| Gtyp gt => [:: gt]
+| Atyp ft' m => let elt_list := list_rhs_type_p ft' in
+                (* append m copies of elt_list to the empty list: *)
+                iter m (fun (ll : seq fgtyp) => ll ++ elt_list) [::]
+| Btyp ff => list_rhs_ffield_p ff
+end
+with list_rhs_ffield_p (ff : ffield) : seq fgtyp :=
+match ff with
+| Fnil => [::]
+| Fflips _ _ ft' ff' => (list_rhs_type_p ft') ++ (list_rhs_ffield_p ff')
+end.
+
+
+(*---------------------------------------------------------------------------*)
+(* Semantics of ports                                                        *)
+
+Definition Sem_frag_port (vm_old : module_graph_vertex_set_p.env) (ct_old : module_graph_connection_trees_p.env) (p : HiFP.hfport) (vm_new : module_graph_vertex_set_p.env) (ct_new : module_graph_connection_trees_p.env) (tmap : CEP.t ftype) : Prop :=
+(* returns True if the port in p defines the components in vm *)
+match p with
+| Finput v t =>
+    match CEP.find v tmap with
+    | Some newft =>
+           (* ground-type input ports are defined *)
+           (forall n : nat,
+                match List.nth_error (list_rhs_type_p newft) n with
+                | Some gt => module_graph_vertex_set_p.find (fst v, N.add (snd v) (N.of_nat n)) vm_new = Some (InPort gt)
+                | None => True
+                end)
+        /\ (* other vertices do not change *)
+           (forall (v0 n0 : N), v0 <> fst v \/ n0 < snd v \/ n0 >= N.add (snd v) (N.of_nat (size_of_ftype newft)) ->
+                module_graph_vertex_set_p.find (v0, n0) vm_old =
+                module_graph_vertex_set_p.find (v0, n0) vm_new)
+        /\ (* connections do not change *)
+           module_graph_connection_trees_p.Equal ct_old ct_new
+    | None => False
+    end
+| Foutput v t =>
+    match CEP.find v tmap with
+    | Some newft =>
+           (* ground-type input ports are defined *)
+           (forall n : nat,
+                match List.nth_error (list_rhs_type_p newft) n with
+                | Some gt => module_graph_vertex_set_p.find (fst v, N.add (snd v) (N.of_nat n)) vm_new = Some (OutPort gt)
+                | None => True
+                end)
+        /\ (* other vertices do not change *)
+           (forall (v0 n0 : N), v0 <> fst v \/ n0 < snd v \/ n0 >= N.add (snd v) (N.of_nat (size_of_ftype newft)) ->
+                module_graph_vertex_set_p.find (v0, n0) vm_old =
+                module_graph_vertex_set_p.find (v0, n0) vm_new)
+        /\ (* other connections do not change *)
+           (forall (v0 n0 o0 : N), v0 <> fst v \/ n0 < snd v \/ n0 >= N.add (snd v) (N.of_nat (size_of_ftype newft)) \/ o0 <> N0 ->
+                module_graph_connection_trees_p.find (v0, n0, o0) ct_old =
+                module_graph_connection_trees_p.find (v0, n0, o0) ct_new)
+        /\ (* set input connectors to undefined *)
+           forall n0 : N, n0 < size_of_ftype newft ->
+               module_graph_connection_trees_p.find (fst v, N.add (snd v) n0, N0) ct_new = Some D_undefined
+    | None => False
+    end
+end.
+
+Fixpoint Sem_frag_ports (vm_old : module_graph_vertex_set_p.env) (ct_old : module_graph_connection_trees_p.env) (pp : seq HiFP.hfport) (vm_new : module_graph_vertex_set_p.env) (ct_new : module_graph_connection_trees_p.env) (tmap : CEP.t ftype) : Prop :=
+(* returns True if the ports in pp define the components in vm *)
+match pp with
+| [::] => vm_old = vm_new /\ ct_old = ct_new
+| p :: pp' =>
+    exists (vm' : module_graph_vertex_set_p.env) (ct' : module_graph_connection_trees_p.env),
+           Sem_frag_port vm_old ct_old p vm' ct' tmap
+        /\
+           Sem_frag_ports vm' ct' pp' vm_new ct_new tmap
+end.
+
+
+(*---------------------------------------------------------------------------*)
+(* Helper functions for connecting                                           *)
+
+Fixpoint connect_type_compatible (can_flip : bool) (ft_tgt ft_src : ftype) (flipped : bool) : bool :=
+(* Returns true if a connection from ft_src to ft_tgt is allowed.
+   flipped == true indicates that the connection should be the other way actually.
+   If can_flip == false, no flipped fields are allowed in bundle types. *)
+match ft_tgt, ft_src with
+| Gtyp (Fuint _), Gtyp (Fuint _)
+| Gtyp (Fsint _), Gtyp (Fsint _)
+| Gtyp Fclock, Gtyp Fclock
+| Gtyp Fasyncreset, Gtyp Fasyncreset => true
+| Gtyp (Fuint_implicit w_tgt), Gtyp (Fuint w_src)
+| Gtyp (Fsint_implicit w_tgt), Gtyp (Fsint w_src) => flipped || (w_tgt >= w_src)
+| Gtyp (Fuint w_tgt), Gtyp (Fuint_implicit w_src)
+| Gtyp (Fsint w_tgt), Gtyp (Fsint_implicit w_src) => (~~flipped) || (w_tgt <= w_src)
+| Gtyp (Fuint_implicit w_tgt), Gtyp (Fuint_implicit w_src)
+| Gtyp (Fsint_implicit w_tgt), Gtyp (Fsint_implicit w_src) =>
+    if flipped then w_tgt <= w_src else w_tgt >= w_src
+| Atyp ft_tgt' n_tgt, Atyp ft_src' n_src =>
+       (n_tgt == n_src)
+    &&
+       connect_type_compatible can_flip ft_tgt' ft_src' flipped
+| Btyp ff_tgt, Btyp ff_src => connect_type_compatible_fields can_flip ff_tgt ff_src flipped
+| _, _ => false
+end
+with connect_type_compatible_fields (can_flip : bool) (ff_tgt ff_src : ffield) (flipped : bool) : bool :=
+(* Returns true if a connection from (Btyp ff_src) to (Btyp ff_tgt) is allowed.
+   flipped == true indicates that the connection should be the other way actually.
+   If can_flip == false, no flipped fields are allowed in bundle types. *)
+match ff_tgt, ff_src with
+| Fnil, Fnil => true
+| Fflips v_tgt Nflip ft_tgt ff_tgt', Fflips v_src Nflip ft_src ff_src' =>
+       (v_tgt == v_src)
+    &&
+       connect_type_compatible can_flip ft_tgt ft_src flipped
+    &&
+       connect_type_compatible_fields can_flip ff_tgt' ff_src' flipped
+| Fflips v_tgt Flipped ft_tgt ff_tgt', Fflips v_src Flipped ft_src ff_src' =>
+       can_flip
+    &&
+       (v_tgt == v_src)
+    &&
+       connect_type_compatible can_flip ft_tgt ft_src (~~flipped)
+    &&
+       connect_type_compatible_fields can_flip ff_tgt' ff_src' flipped
+| _, _ => false
+end.
+
+Definition connect_fgtyp (ct_old : module_graph_connection_trees_p.env)
+                         (ref_tgt : HiFP.href) (lst_tgt : list PProdVarOrder.t)
+                         (ref_src : HiFP.href) (lst_src : list PProdVarOrder.t)
+                         (flipped : bool)
+                         (ct_new : module_graph_connection_trees_p.env) : bool :=
+(* The predicate checks whether ct_new contains the correct connection that connects from lst_src to lst_tgt,
+   and it does not change the connection into lst_src.
+   These lists must be one-element lists for output and input connectors of compatible types.
+   It assumes that the types are compatible. *)
+match flipped, ref_tgt, lst_tgt, ref_src, lst_src with
+| false, _, [:: ic], ref_src, [:: oc]
+| true,  ref_src, [:: oc], _, [:: ic] =>
+       (module_graph_connection_trees_p.find ic ct_new == Some (D_fexpr (Eref ref_src)))
+    &&
+       (module_graph_connection_trees_p.find oc ct_new == module_graph_connection_trees_p.find oc ct_old)
+       (* why this is compared?
+          In Sem_frag_stmt, it is ensured that connection trees NOT related to tgt or src are not changed.
+          Here, we need to ensure that the connection tree of tgt is changed
+          and the connection tree of src remains the same. *)
+| _, _, _, _, _ => false
+end.
+
+Fixpoint connect (ct_old : module_graph_connection_trees_p.env)
+                 (ref_tgt : HiFP.href) (lst_tgt : list PProdVarOrder.t) (ft_tgt : ftype)
+                 (ref_src : HiFP.href) (lst_src : list PProdVarOrder.t) (ft_src : ftype)
+                 (flipped : bool)
+                 (ct_new : module_graph_connection_trees_p.env) : bool :=
+(* The predicate returns true if the correct connection trees are in ct_new
+   that connect from lst_src to lst_tgt, and that the connection trees that
+   connect to lst_src are not changed.  Other connection trees are not checked.
+   The type of lst_tgt is ft_tgt, and the type of lst_src is ft_src.
+   These references are *not* required to have passive types. *)
+match ft_tgt, ft_src with
+| Gtyp gt_tgt, Gtyp gt_src => connect_fgtyp ct_old ref_tgt lst_tgt ref_src lst_src flipped ct_new
+| Atyp elt_tgt n1, Atyp elt_src n2 =>
+       (n1 == n2)
+   &&
+       let type_len := size_of_ftype elt_tgt in
+       [forall n : ordinal n1,
+          connect ct_old
+                  (Esubindex ref_tgt n) (take type_len (drop (n * type_len) lst_tgt)) elt_tgt
+                  (Esubindex ref_src n) (take type_len (drop (n * type_len) lst_src)) elt_src
+                  flipped ct_new]
+| Btyp ff_tgt, Btyp ff_src => connect_fields ct_old ref_tgt lst_tgt ff_tgt ref_src lst_src ff_src flipped ct_new
+| _, _ => false
+end
+with connect_fields (ct_old : module_graph_connection_trees_p.env)
+                    (ref_tgt : HiFP.href) (lst_tgt : list PProdVarOrder.t) (ft_tgt : ffield)
+                    (ref_src : HiFP.href) (lst_src : list PProdVarOrder.t) (ft_src : ffield)
+                    (flipped : bool)
+                    (ct_new : module_graph_connection_trees_p.env) : bool :=
+(* The predicate returns true if the correct connection trees are in ct_new
+   that connect from lst_src to lst_tgt, and that the connection trees that
+   connect to lst_src are not changed.  Other connection trees are not checked.
+   The type of lst_tgt is (Btyp ft_tgt), and the type of lst_src is (Btyp ft_src).
+   These references are *not* required to have passive types. *)
+match ft_tgt, ft_src with
+| Fnil, Fnil => true
+| Fflips v1 Nflip gtt ft, Fflips v2 Nflip gts fs =>
+       (v1 == v2)
+    &&
+       let type_len := size_of_ftype gtt in
+              connect ct_old (Esubfield ref_tgt v1) (take type_len lst_tgt) gtt (Esubfield ref_src v2) (take type_len lst_src) gts flipped ct_new
+           &&
+              connect_fields ct_old ref_tgt (drop type_len lst_tgt) ft ref_src (drop type_len lst_src) fs flipped ct_new
+| Fflips v1 Flipped gtt ft, Fflips v2 Flipped gts fs =>
+       (v1 == v2)
+    &&
+       let type_len := size_of_ftype gts in
+              connect ct_old (Esubfield ref_tgt v1) (take type_len lst_tgt) gtt (Esubfield ref_src v2) (take type_len lst_src) gts (~~flipped) ct_new
+           &&
+              connect_fields ct_old ref_tgt (drop type_len lst_tgt) ft ref_src (drop type_len lst_src) fs flipped ct_new
+| _, _ => false
 end.
 
 Fixpoint ftype_is_passive (ft : ftype) : bool :=
@@ -938,7 +1435,11 @@ match d_true, d_false with
 | _, Some D_undefined => d_false
 end.
 
-Fixpoint Sem_frag_stmt (vm_old : module_graph_vertex_set_p.env) (ct_old : module_graph_connection_trees_p.env) (s : HiFP.hfstmt) (vm_new : module_graph_vertex_set_p.env) (ct_new : module_graph_connection_trees_p.env) (tmap : ft_pmap) : Prop :=
+
+(*---------------------------------------------------------------------------*)
+(* Semantics of statements                                                   *)
+
+Fixpoint Sem_frag_stmt (vm_old : module_graph_vertex_set_p.env) (ct_old : module_graph_connection_trees_p.env) (s : HiFP.hfstmt) (vm_new : module_graph_vertex_set_p.env) (ct_new : module_graph_connection_trees_p.env) (tmap : CEP.t ftype) : Prop :=
    (* The predicate returns True if vm_new/ct_new can be constructed from vm_old/ct_old by applying s.
    type checking, constraints *)
    match s with
@@ -948,7 +1449,9 @@ Fixpoint Sem_frag_stmt (vm_old : module_graph_vertex_set_p.env) (ct_old : module
        /\
           match list_lhs_ref_p ref_tgt tmap, list_lhs_ref_p ref_src tmap with
           | Some (lst_tgt, ft_tgt), Some (lst_src, ft_src) =>
-                 connect_non_passive ct_old ref_tgt lst_tgt ft_tgt ref_src lst_src ft_src ct_new
+                 connect_type_compatible true ft_tgt ft_src false
+              /\
+                 connect ct_old ref_tgt lst_tgt ft_tgt ref_src lst_src ft_src false ct_new
               /\
                  forall v0 : PProdVarOrder.T,
                     if (v0 \in lst_tgt) || (v0 \in lst_src) then True (* already checked in connect_non_passive *)
@@ -959,10 +1462,10 @@ Fixpoint Sem_frag_stmt (vm_old : module_graph_vertex_set_p.env) (ct_old : module
           module_graph_vertex_set_p.Equal vm_old vm_new
        /\
           match list_lhs_ref_p ref tmap, type_of_expr expr tmap with
-          | Some (input_list, ft_ref), Some ft_expr =>
-                 connect_type_compatible ft_ref ft_expr
+          | Some (input_list, ft_ref), Some (exist ft_expr _) =>
+                 connect_type_compatible false ft_ref ft_expr false
               /\
-                 match list_rhs_expr_p expr (proj1_sig ft_expr) with
+                 match list_rhs_expr_p expr ft_expr with
                  | Some expr_list =>
                         (forall n : nat,
                              match List.nth_error input_list n, List.nth_error expr_list n with
@@ -996,70 +1499,83 @@ Fixpoint Sem_frag_stmt (vm_old : module_graph_vertex_set_p.env) (ct_old : module
                      else module_graph_connection_trees_p.find v0 ct_old = module_graph_connection_trees_p.find v0 ct_new
           | _ => False
           end
-   | Swire v t =>
-       match t with
-       | Gtyp oldgt => (* only v changes *)
-           if module_graph_vertex_set_p.find v vm_new is Some (Wire newgt)
-           then    module_graph_vertex_set_p.Equal (module_graph_vertex_set_p.add v (Wire newgt) vm_old) vm_new
-                /\
-                   module_graph_connection_trees_p.Equal (module_graph_connection_trees_p.add (v, N0) D_undefined ct_old) ct_new
-                /\
-                   vtype_equivalent oldgt newgt
-           else False
-       | _ => (* (fst v, N0), ... all have changed *)
-           (* find the type of (fst v, N0), ..., (fst v, ...) based on t. *)
-           if vtype_find_widths t (fst v) N0 vm_new is Some (newft, newft_size)
-           then    (* ground-type wires are defined *)
-                   (forall n : nat,
-                        match List.nth_error (list_rhs_type_p newft) n with
-                        | Some gt => module_graph_vertex_set_p.find (fst v, N.of_nat n) vm_new = Some (Wire gt)
-                        | None => True
-                        end)
-                /\ (* other vertices do not change *)
-                   (forall (v0 n0 : N), v0 <> fst v \/ n0 >= newft_size ->
-                        module_graph_vertex_set_p.find (v0, n0) vm_old =
-                        module_graph_vertex_set_p.find (v0, n0) vm_new)
-                /\ (* other connections do not change *)
-                   (forall (v0 n0 o0 : N), v0 <> fst v \/ n0 >= newft_size \/ o0 > 0 ->
-                        module_graph_connection_trees_p.find (v0, n0, o0) ct_old =
-                        module_graph_connection_trees_p.find (v0, n0, o0) ct_new)
-                /\ (* set wires to undefined *)
-                   forall n0 : N, n0 < newft_size ->
-                       module_graph_connection_trees_p.find (fst v, n0, N0) ct_new = Some D_undefined
-           else False
+   | Swire v _ =>
+       match CEP.find v tmap with
+       | Some newft =>
+              (* ground-type wires are defined *)
+              (forall n : nat,
+                   match List.nth_error (list_rhs_type_p newft) n with
+                   | Some gt => module_graph_vertex_set_p.find (fst v, N.add (snd v) (N.of_nat n)) vm_new = Some (Wire gt)
+                   | None => True
+                   end)
+           /\ (* other vertices do not change *)
+              (forall (v0 n0 : N), v0 <> fst v \/ n0 < snd v \/ n0 >= N.add (snd v) (N.of_nat (size_of_ftype newft)) ->
+                   module_graph_vertex_set_p.find (v0, n0) vm_old =
+                   module_graph_vertex_set_p.find (v0, n0) vm_new)
+           /\ (* other connections do not change *)
+              (forall (v0 n0 o0 : N), v0 <> fst v \/ n0 < snd v \/ n0 >= N.add (snd v) (N.of_nat (size_of_ftype newft)) \/ o0 <> N0 ->
+                   module_graph_connection_trees_p.find (v0, n0, o0) ct_old =
+                   module_graph_connection_trees_p.find (v0, n0, o0) ct_new)
+           /\ (* set wires to undefined *)
+              forall n0 : N, n0 < size_of_ftype newft ->
+                  module_graph_connection_trees_p.find (fst v, N.add (snd v) n0, N0) ct_new = Some D_undefined
+       | None => False (* should not happen *)
        end
    | Sreg v reg =>
-       match type reg, module_graph_vertex_set_p.find v vm_new with
-       | Gtyp oldgt, Some (Register newgt)
-       | Gtyp oldgt, Some (RegisterReset newgt _) => (* ground-type register, only v changes *)
+       match CEP.find v tmap with
+       | Some newft => (* aggregate-type register *)
               match reset reg with
               | Rst rst_sig rst_val =>
                      (* type check rst_sig *)
                      match type_of_expr rst_sig tmap with
                      | Some (exist (Gtyp (Fuint 1)) _) =>
-                         (* module graph contains register with synchronous reset *)
-                         module_graph_vertex_set_p.Equal (module_graph_vertex_set_p.add v (RegisterReset newgt false) vm_old) vm_new
+                         (* module graph contains ground-type registers with synchronous reset *)
+                         forall n : nat,
+                             match List.nth_error (list_rhs_type_p newft) n with
+                             | Some gt => module_graph_vertex_set_p.find (fst v, N.add (snd v) (N.of_nat n)) vm_new = Some (RegisterReset gt false)
+                             | None => True
+                             end
                      | Some (exist (Gtyp Fasyncreset) _) =>
-                         (* module graph contains register with asynchronous reset *)
-                         module_graph_vertex_set_p.Equal (module_graph_vertex_set_p.add v (RegisterReset newgt true) vm_old) vm_new
+                         (* module graph contains ground-type registers with asynchronous reset *)
+                         forall n : nat,
+                             match List.nth_error (list_rhs_type_p newft) n with
+                             | Some gt => module_graph_vertex_set_p.find (fst v, N.add (snd v) (N.of_nat n)) vm_new = Some (RegisterReset gt true)
+                             | None => True
+                             end
                      | _ => False
                      end
                   /\ (* connect rst_sig *)
-                     module_graph_connection_trees_p.find (v, 2%num) ct_new = Some (D_fexpr rst_sig)
-                  /\ (* type check rst_val *)
+                     (forall n0 : N, n0 < size_of_ftype newft ->
+                         module_graph_connection_trees_p.find (fst v, N.add (snd v) n0, 2%num) ct_new = Some (D_fexpr rst_sig))
+                  /\ (* type check rst_val -- also ensures that newft is passive *)
                      match type_of_expr rst_val tmap with
-                     | Some rst_val_type => connect_type_compatible (Gtyp newgt) rst_val_type
+                     | Some (exist rst_val_type _) => connect_type_compatible false newft rst_val_type false
                      | None => False
                      end
                   /\ (* connect rst_val *)
-                     module_graph_connection_trees_p.find (v, 3%num) ct_new = Some (D_fexpr rst_val)
+                     match list_rhs_expr_p rst_val newft with
+                     | Some expr_list =>
+                         forall n : nat,
+                             match List.nth_error expr_list n with
+                             | Some ex => module_graph_connection_trees_p.find (fst v, N.add (snd v) (N.of_nat n), 3%num) ct_new = Some (D_fexpr ex)
+                             | None => True
+                             end
+                     | None => False
+                     end
               | NRst =>
-                     (* module graph contains register without reset *)
-                     module_graph_vertex_set_p.Equal (module_graph_vertex_set_p.add v (Register newgt) vm_old) vm_new
+                     (* module graph contains ground-type registers without reset *)
+                     (forall n : nat,
+                          match List.nth_error (list_rhs_type_p newft) n with
+                          | Some gt => module_graph_vertex_set_p.find (fst v, N.add (snd v) (N.of_nat n)) vm_new = Some (Register gt)
+                          | None => True
+                          end)
                   /\ (* input connectors reserved for rst_sig and rst_val do not change *)
-                     module_graph_connection_trees_p.find (v, 2%num) ct_old = module_graph_connection_trees_p.find (v, 2%num) ct_new
-                  /\
-                     module_graph_connection_trees_p.find (v, 3%num) ct_old = module_graph_connection_trees_p.find (v, 3%num) ct_new
+                     (forall n0 : N, n0 < size_of_ftype newft ->
+                             module_graph_connection_trees_p.find (fst v, N.add (snd v) n0, 2%num) ct_old = module_graph_connection_trees_p.find (fst v, N.add (snd v) n0, 2%num) ct_new
+                          /\
+                             module_graph_connection_trees_p.find (fst v, N.add (snd v) n0, 3%num) ct_old = module_graph_connection_trees_p.find (fst v, N.add (snd v) n0, 3%num) ct_new)
+                  /\ (* type check newft: we only need to verify newft is passive *)
+                     ftype_is_passive newft
               end
            /\ (* type check clock *)
               match type_of_expr (clock reg) tmap with
@@ -1067,122 +1583,43 @@ Fixpoint Sem_frag_stmt (vm_old : module_graph_vertex_set_p.env) (ct_old : module
               | _ => False
               end
            /\ (* connect clock *)
-              module_graph_connection_trees_p.find (v, 1%num) ct_new = Some (D_fexpr (clock reg))
+              (forall n0 : N, n0 < size_of_ftype newft ->
+                  module_graph_connection_trees_p.find (fst v, N.add (snd v) n0, 1%num) ct_new = Some (D_fexpr (clock reg)))
            /\ (* connect default value for register *)
-              module_graph_connection_trees_p.find (v, N0) ct_new = Some (D_fexpr (Eref (Eid v)))
+              match list_rhs_expr_p (Eref (Eid v)) newft with
+              | Some expr_list =>
+                  forall n : nat,
+                      match List.nth_error expr_list n with
+                      | Some ex => module_graph_connection_trees_p.find (fst v, N.add (snd v) (N.of_nat n), N0) ct_new = Some (D_fexpr ex)
+                      | None => True
+                      end
+              | None => False
+              end
+           /\ (* other vertices do not change *)
+              (forall (v0 n0 : N), v0 <> fst v \/ n0 < snd v \/ n0 >= N.add (snd v) (N.of_nat (size_of_ftype newft)) ->
+                  module_graph_vertex_set_p.find (v0, n0) vm_old =
+                  module_graph_vertex_set_p.find (v0, n0) vm_new)
            /\ (* other connections do not change *)
-              (forall (v0 : ProdVarOrder.T) (o0 : N), v0 <> v \/ o0 > 3 ->
-                  module_graph_connection_trees_p.find (v0, o0) ct_old =
-                  module_graph_connection_trees_p.find (v0, o0) ct_new)
-           /\ (* type check newgt *)
-              vtype_equivalent oldgt newgt
-       | Gtyp _, _ => False (* module graph does not contain correct component *)
-       | _, _ => (* aggregate-type register *)
-           if vtype_find_widths (type reg) (fst v) N0 vm_new is Some (newft, newft_size)
-           then    match reset reg with
-                   | Rst rst_sig rst_val =>
-                          (* type check rst_sig *)
-                          match type_of_expr rst_sig tmap with
-                          | Some (exist (Gtyp (Fuint 1)) _) =>
-                              (* module graph contains ground-type registers with synchronous reset *)
-                              forall n : nat,
-                                  match List.nth_error (list_rhs_type_p newft) n with
-                                  | Some gt => module_graph_vertex_set_p.find (fst v, N.of_nat n) vm_new = Some (RegisterReset gt false)
-                                  | None => True
-                                  end
-                          | Some (exist (Gtyp Fasyncreset) _) =>
-                              (* module graph contains ground-type registers with asynchronous reset *)
-                              forall n : nat,
-                                  match List.nth_error (list_rhs_type_p newft) n with
-                                  | Some gt => module_graph_vertex_set_p.find (fst v, N.of_nat n) vm_new = Some (RegisterReset gt true)
-                                  | None => True
-                                  end
-                          | _ => False
-                          end
-                       /\ (* connect rst_sig *)
-                          (forall n0 : N, n0 < newft_size ->
-                              module_graph_connection_trees_p.find (fst v, n0, 2%num) ct_new = Some (D_fexpr rst_sig))
-                       /\ (* type check rst_val -- also ensures that newft is passive *)
-                          match type_of_expr rst_val tmap with
-                          | Some rst_val_type => connect_type_compatible newft rst_val_type
-                          | None => False
-                          end
-                       /\ (* connect rst_val *)
-                          match list_rhs_expr_p rst_val newft with
-                          | Some expr_list =>
-                              forall n : nat,
-                                  match List.nth_error expr_list n with
-                                  | Some ex => module_graph_connection_trees_p.find (fst v, N.of_nat n, 3%num) ct_new = Some (D_fexpr ex)
-                                  | None => True
-                                  end
-                          | None => False
-                          end
-                   | NRst =>
-                          (* module graph contains ground-type registers without reset *)
-                          (forall n : nat,
-                               match List.nth_error (list_rhs_type_p newft) n with
-                               | Some gt => module_graph_vertex_set_p.find (fst v, N.of_nat n) vm_new = Some (Register gt)
-                               | None => True
-                               end)
-                       /\ (* input connectors reserved for rst_sig and rst_val do not change *)
-                          (forall n0 : N, n0 < newft_size ->
-                                  module_graph_connection_trees_p.find (fst v, n0, 2%num) ct_old = module_graph_connection_trees_p.find (fst v, n0, 2%num) ct_new
-                               /\
-                                  module_graph_connection_trees_p.find (fst v, n0, 3%num) ct_old = module_graph_connection_trees_p.find (fst v, n0, 3%num) ct_new)
-                       /\ (* type check newft: most has been done by vtype_find_widths, we only need to ensure newft is passive *)
-                          ftype_is_passive newft
-                   end
-                /\ (* type check clock *)
-                   match type_of_expr (clock reg) tmap with
-                   | Some (exist (Gtyp Fclock) _) => True
-                   | _ => False
-                   end
-                /\ (* connect clock *)
-                   (forall n0 : N, n0 < newft_size ->
-                       module_graph_connection_trees_p.find (fst v, n0, 1%num) ct_new = Some (D_fexpr (clock reg)))
-                /\ (* connect default value for register *)
-                   match list_rhs_expr_p (Eref (Eid v)) newft with
-                   | Some expr_list =>
-                       forall n : nat,
-                           match List.nth_error expr_list n with
-                           | Some ex => module_graph_connection_trees_p.find (fst v, N.of_nat n, N0) ct_new = Some (D_fexpr ex)
-                           | None => True
-                           end
-                   | None => False
-                   end
-                /\ (* other vertices do not change *)
-                   (forall (v0 n0 : N), v0 <> fst v \/ n0 >= newft_size ->
-                       module_graph_vertex_set_p.find (v0, n0) vm_old =
-                       module_graph_vertex_set_p.find (v0, n0) vm_new)
-                /\ (* other connections do not change *)
-                   (forall (v0 n0 o0 : N), v0 <> fst v \/ n0 >= newft_size \/ o0 > 3 ->
-                       module_graph_connection_trees_p.find (v0, n0, o0) ct_old =
-                       module_graph_connection_trees_p.find (v0, n0, o0) ct_new)
-           else False
+              (forall (v0 n0 o0 : N), v0 <> fst v \/ n0 < snd v \/ n0 >= N.add (snd v) (N.of_nat (size_of_ftype newft)) \/ o0 > 3%num ->
+                  module_graph_connection_trees_p.find (v0, n0, o0) ct_old =
+                  module_graph_connection_trees_p.find (v0, n0, o0) ct_new)
+       | None => False (* should not happen *)
        end
    | Snode v expr =>
        match type_of_expr expr tmap with
-       | Some (exist (Gtyp oldgt) _) => (* only v changes *)
-           if module_graph_vertex_set_p.find v vm_new is Some (Node newgt)
-           then    module_graph_vertex_set_p.Equal (module_graph_vertex_set_p.add v (Node newgt) vm_old) vm_new
-                /\
-                   module_graph_connection_trees_p.Equal (module_graph_connection_trees_p.add (v, N0) (D_fexpr expr) ct_old) ct_new
-                /\
-                   vtype_equivalent oldgt newgt
-           else False
        | Some (exist newft _) => (* (fst v, N0), ... all have changed *)
               (* ground-type nodes are defined *)
               (forall n : nat,
                    match List.nth_error (list_rhs_type_p newft) n with
-                   | Some gt => module_graph_vertex_set_p.find (fst v, N.of_nat n) vm_new = Some (Node gt)
+                   | Some gt => module_graph_vertex_set_p.find (fst v, N.add (snd v) (N.of_nat n)) vm_new = Some (Node gt)
                    | None => True
                    end)
            /\ (* other vertices do not change *)
-              (forall (v0 n0 : N), v0 <> fst v \/ n0 >= size_of_ftype newft ->
+              (forall (v0 n0 : N), v0 <> fst v \/ n0 < snd v \/ n0 >= N.add (snd v) (N.of_nat (size_of_ftype newft)) ->
                    module_graph_vertex_set_p.find (v0, n0) vm_old =
                    module_graph_vertex_set_p.find (v0, n0) vm_new)
            /\ (* other connections do not change *)
-              (forall (v0 n0 o0 : N), v0 <> fst v \/ n0 >= size_of_ftype newft \/ o0 > 0 ->
+              (forall (v0 n0 o0 : N), v0 <> fst v \/ n0 < snd v \/ n0 >= N.add (snd v) (N.of_nat (size_of_ftype newft)) \/ o0 <> N0 ->
                    module_graph_connection_trees_p.find (v0, n0, o0) ct_old =
                    module_graph_connection_trees_p.find (v0, n0, o0) ct_new)
            /\ (* set nodes to the respective part of the expression *)
@@ -1190,7 +1627,7 @@ Fixpoint Sem_frag_stmt (vm_old : module_graph_vertex_set_p.env) (ct_old : module
               | Some expr_list =>
                   forall n : nat,
                       match List.nth_error expr_list n with
-                      | Some ex => module_graph_connection_trees_p.find (fst v, N.of_nat n, N0) ct_new = Some (D_fexpr ex)
+                      | Some ex => module_graph_connection_trees_p.find (fst v, N.add (snd v) (N.of_nat n), N0) ct_new = Some (D_fexpr ex)
                       | None => True
                       end
               | None => False
@@ -1210,7 +1647,7 @@ Fixpoint Sem_frag_stmt (vm_old : module_graph_vertex_set_p.env) (ct_old : module
                        (module_graph_connection_trees_p.map2 (Swhen_map2_helper cond) ct_true ct_false)
        else False
 end
-with Sem_frag_stmts (vm_old : module_graph_vertex_set_p.env) (ct_old : module_graph_connection_trees_p.env) (ss : HiFP.hfstmt_seq) (vm_new : module_graph_vertex_set_p.env) (ct_new : module_graph_connection_trees_p.env) (tmap : ft_pmap) : Prop :=
+with Sem_frag_stmts (vm_old : module_graph_vertex_set_p.env) (ct_old : module_graph_connection_trees_p.env) (ss : HiFP.hfstmt_seq) (vm_new : module_graph_vertex_set_p.env) (ct_new : module_graph_connection_trees_p.env) (tmap : CEP.t ftype) : Prop :=
 match ss with
 | Qnil =>
        module_graph_vertex_set_p.Equal vm_old vm_new
@@ -1223,438 +1660,9 @@ match ss with
            Sem_frag_stmts vm' ct' ss' vm_new ct_new tmap
 end.
 
-Definition Sem_frag_port (vm_old : module_graph_vertex_set_p.env) (ct_old : module_graph_connection_trees_p.env) (p : HiFP.hfport) (vm_new : module_graph_vertex_set_p.env) (ct_new : module_graph_connection_trees_p.env) : Prop :=
-(* returns True if the port in p defines the components in vm *)
-match p with
-| Finput v t =>
-    match t with
-    | Gtyp ft =>
-           module_graph_vertex_set_p.Equal (module_graph_vertex_set_p.add v (InPort ft) vm_old) vm_new
-        /\
-           module_graph_connection_trees_p.Equal ct_old ct_new
-    | _ =>
-        if vtype_find_widths t (fst v) N0 vm_new is Some (newft, newft_size)
-        then    (* ground-type input ports are defined *)
-                (forall n : nat,
-                     match List.nth_error (list_rhs_type_p newft) n with
-                     | Some gt => module_graph_vertex_set_p.find (fst v, N.of_nat n) vm_new = Some (InPort gt)
-                     | None => True
-                     end)
-             /\ (* other vertices do not change *)
-                (forall (v0 n0 : N), v0 <> fst v \/ n0 >= newft_size ->
-                     module_graph_vertex_set_p.find (v0, n0) vm_old =
-                     module_graph_vertex_set_p.find (v0, n0) vm_new)
-             /\ (* connections do not change *)
-                module_graph_connection_trees_p.Equal ct_old ct_new
-        else False
-    end
-| Foutput v t =>
-    match t with
-    | Gtyp ft =>
-           module_graph_vertex_set_p.Equal (module_graph_vertex_set_p.add v (OutPort ft) vm_old) vm_new
-        /\
-           module_graph_connection_trees_p.Equal (module_graph_connection_trees_p.add (v, N0) D_undefined ct_old) ct_new
-    | _ =>
-        if vtype_find_widths t (fst v) N0 vm_new is Some (newft, newft_size)
-        then    (* ground-type input ports are defined *)
-                (forall n : nat,
-                     match List.nth_error (list_rhs_type_p newft) n with
-                     | Some gt => module_graph_vertex_set_p.find (fst v, N.of_nat n) vm_new = Some (OutPort gt)
-                     | None => True
-                     end)
-             /\ (* other vertices do not change *)
-                (forall (v0 n0 : N), v0 <> fst v \/ n0 >= newft_size ->
-                     module_graph_vertex_set_p.find (v0, n0) vm_old =
-                     module_graph_vertex_set_p.find (v0, n0) vm_new)
-             /\ (* other connections do not change *)
-                (forall (v0 n0 o0 : N), v0 <> fst v \/ n0 >= newft_size \/ o0 > 0 ->
-                     module_graph_connection_trees_p.find (v0, n0, o0) ct_old =
-                     module_graph_connection_trees_p.find (v0, n0, o0) ct_new)
-             /\ (* set wires to undefined *)
-                forall n0 : N, n0 < newft_size ->
-                    module_graph_connection_trees_p.find (fst v, n0, N0) ct_new = Some D_undefined
-        else False
-    end
-end.
 
-Fixpoint Sem_frag_ports (vm_old : module_graph_vertex_set_p.env) (ct_old : module_graph_connection_trees_p.env) (pp : seq HiFP.hfport) (vm_new : module_graph_vertex_set_p.env) (ct_new : module_graph_connection_trees_p.env) : Prop :=
-(* returns True if the ports in pp define the components in vm *)
-match pp with
-| [::] => vm_old = vm_new /\ ct_old = ct_new
-| p :: pp' =>
-    exists (vm' : module_graph_vertex_set_p.env) (ct' : module_graph_connection_trees_p.env),
-           Sem_frag_port vm_old ct_old p vm' ct'
-        /\
-           Sem_frag_ports vm' ct' pp' vm_new ct_new
-end.
-
-Fixpoint ports_tmap (pp : seq HiFP.hfport) : ft_pmap :=
-(* creates a tmap that contains exactly the types of the ports in pp. *)
-match pp with
-| [::] => ft_empty
-| Finput v t :: pp'
-| Foutput v t :: pp' => ft_add v t (ports_tmap pp')
-end.
-
-Fixpoint stmts_tmap (tmap_scope : ft_pmap * ft_pmap) (ss : HiFP.hfstmt_seq) : option (ft_pmap * ft_pmap) :=
-(* extends tmap_scope with the types of the defined components in ss.
-   The first part of tmap_scope contains all defined components
-   (used to check for name clashes, and will also be used later in Sem_frag_stmt);
-   the second part contains only the components in the current scope
-   (used to check whether a component defined within a Swhen statement
-   is illegally used outside it).
-   Produces None if some component is defined more than once,
-   if a component is accessed before it is defined,
-   or if it is accessed out of scope.
-
-   Problem: does not check the directionality of the component
-   (e.g. a node can only be read, an output port can only be written).
-   Should we replace the tmap with a component environment? *)
-match ss with
-| Qnil => Some tmap_scope
-| Qcons s ss' =>
-    match stmt_tmap tmap_scope s with
-    | Some tmap_scope' => stmts_tmap tmap_scope' ss'
-    | None => None
-    end
-end
-with stmt_tmap (tmap_scope : ft_pmap * ft_pmap) (s : HiFP.hfstmt) : option (ft_pmap * ft_pmap) :=
-(* extends tmap_scope with the type of the component defined in s.
-   Produces None if s contains a definition of a component that is already in tmap. *)
-match s with
-| Sskip => Some tmap_scope
-| Sfcnct ref expr =>
-    match type_of_ref ref (snd tmap_scope), type_of_expr expr (snd tmap_scope) with
-    | Some _, Some _ => Some tmap_scope
-    | _, _ => None (* something undefined or out-of-scope is accessed *)
-    end
-| Sinvalid ref =>
-    match type_of_ref ref (snd tmap_scope) with
-    | Some _ => Some tmap_scope
-    | None => None (* ref is undefined or out of scope *)
-    end
-| Swire v t =>
-    if ft_find v (fst tmap_scope) == None
-    then Some (ft_add v t (fst tmap_scope), ft_add v t (snd tmap_scope))
-    else None
-| Sreg v reg =>
-    if ft_find v (fst tmap_scope) == None
-    then if reset reg is Rst rst_sig rst_val
-         then match type_of_expr rst_sig (snd tmap_scope), type_of_expr rst_val (snd tmap_scope) with
-              | Some _, Some _ => Some (ft_add v (type reg) (fst tmap_scope), ft_add v (type reg) (snd tmap_scope))
-              | _, _ => None (* something undefined or out-of-scope is accessed *)
-              end
-         else Some (ft_add v (type reg) (fst tmap_scope), ft_add v (type reg) (snd tmap_scope))
-    else None
-| Snode v expr =>
-    match type_of_expr expr (snd tmap_scope) with
-    | Some (exist t _) =>
-        if ft_find v (fst tmap_scope) == None
-        then Some (ft_add v t (fst tmap_scope), ft_add v t (snd tmap_scope))
-        else None
-    | None => None (* something undefined or out-of-scope is accessed *)
-    end
-| Smem _ _ => None
-| Sinst _ _ => None
-| Swhen _ ss_true ss_false =>
-    match stmts_tmap tmap_scope ss_true with
-    | Some (tmap_true, _) =>
-        match stmts_tmap (tmap_true, snd tmap_scope) ss_false with
-        | Some (tmap_false, _) =>
-            Some (tmap_false, snd tmap_scope)
-        | None => None
-        end
-    | None => None
-    end
-end.
-
-Lemma stmts_tmap_subset :
-   forall (ss : HiFP.hfstmt_seq) (tmap scope : ft_pmap),
-      tmap_subset scope tmap ->
-         match stmts_tmap (tmap, scope) ss with
-         | Some (tmap', scope') => tmap_subset scope' tmap' /\ tmap_subset tmap tmap' /\ tmap_subset scope scope'
-         | None => True
-         end
-with stmt_tmap_subset :
-   forall (s : HiFP.hfstmt) (tmap scope : ft_pmap),
-      tmap_subset scope tmap ->
-         match stmt_tmap (tmap, scope) s with
-         | Some (tmap', scope') => tmap_subset scope' tmap' /\ tmap_subset tmap tmap' /\ tmap_subset scope scope'
-         | None => True
-         end.
-Proof.
-* clear stmts_tmap_subset.
-  induction ss.
-  + unfold stmts_tmap.
-    intros ; split ; first by exact H.
-    by split ; apply tmap_subset_refl.
-  + intros.
-    simpl stmts_tmap.
-    specialize stmt_tmap_subset with (s := h) (tmap := tmap) (scope := scope).
-    destruct (stmt_tmap (tmap, scope) h) as [[tmap' scope']|] ; last by trivial.
-    specialize IHss with (tmap := tmap') (scope := scope').
-    destruct (stmts_tmap (tmap', scope') ss) as [[tmap'' scope'']|] ; last by trivial.
-    split.
-    - apply IHss, stmt_tmap_subset, H.
-    split.
-    - apply (tmap_subset_trans tmap') ; first by apply stmt_tmap_subset.
-      by apply IHss, stmt_tmap_subset, H.
-    - apply (tmap_subset_trans scope') ; first by apply stmt_tmap_subset.
-      by apply IHss, stmt_tmap_subset, H.
-* clear stmt_tmap_subset.
-  intro.
-  destruct s ; simpl ; intros ; try trivial.
-  + (* Sskip *) split ; first by exact H.
-    by split ; apply tmap_subset_refl.
-  + (* Swire *)
-    destruct (ft_find s tmap) eqn: Hfind ; simpl ; first by trivial.
-    split.
-    - by apply tmap_subset_add_add, H.
-    split.
-    - by apply tmap_subset_add, Hfind.
-    - apply tmap_subset_add.
-      unfold tmap_subset in H ; specialize H with (v := s).
-      destruct (ft_find s scope) ; last by trivial.
-      by rewrite -H -Hfind //.
-  + (* Sreg *)
-    destruct (ft_find s tmap) eqn: Hfind ; simpl ; first by trivial.
-    destruct (reset h).
-    - split.
-      * by apply tmap_subset_add_add, H.
-      split.
-      * by apply tmap_subset_add, Hfind.
-      * apply tmap_subset_add.
-        unfold tmap_subset in H ; specialize H with (v := s).
-        destruct (ft_find s scope) ; last by trivial.
-        by rewrite -H -Hfind //.
-    - destruct (type_of_expr h0 scope) ; last by trivial.
-      destruct (type_of_expr h1 scope) ; last by trivial.
-      split.
-      * by apply tmap_subset_add_add, H.
-      split.
-      * by apply tmap_subset_add, Hfind.
-      * apply tmap_subset_add.
-        unfold tmap_subset in H ; specialize H with (v := s).
-        destruct (ft_find s scope) ; last by trivial.
-        by rewrite -H -Hfind //.
-  + (* Snode *)
-    destruct (type_of_expr h scope) as [[t p]|] ; last by trivial.
-    destruct (ft_find s tmap) eqn: Hfind ; simpl ; first by trivial.
-    split.
-    - by apply tmap_subset_add_add, H.
-    split.
-    - by apply tmap_subset_add, Hfind.
-    - apply tmap_subset_add.
-      unfold tmap_subset in H ; specialize H with (v := s).
-      destruct (ft_find s scope) ; last by trivial.
-      by rewrite -H -Hfind //.
-  + (* Sfcnct *)
-    destruct (type_of_ref h scope) ; last by trivial.
-    destruct (type_of_expr h0 scope) ; last by trivial.
-    split.
-    - by exact H.
-    - split ; by apply tmap_subset_refl.
-  + (* Sinvalid *)
-    destruct (type_of_ref h scope) ; last by trivial.
-    split.
-    - by exact H.
-    - split ; by apply tmap_subset_refl.
-  + (* Swhen *)
-    rename h0 into ss_true ; rename h1 into ss_false.
-    generalize (stmts_tmap_subset ss_true tmap scope H) ; intro.
-    destruct (stmts_tmap (tmap, scope) ss_true) as [[tmap_true scope_true]|] ; last by trivial.
-    generalize (stmts_tmap_subset ss_false tmap_true scope (tmap_subset_trans tmap _ _ H (proj1 (proj2 H0)))) ; intro.
-    destruct (stmts_tmap (tmap_true, scope) ss_false) as [[tmap_false scope_false]|] ; last by trivial.
-    split.
-    - apply (tmap_subset_trans tmap) ; first by apply H.
-      apply (tmap_subset_trans tmap_true) ; first by apply H0.
-      apply H1.
-    split.
-    - apply (tmap_subset_trans tmap_true) ; first by apply H0.
-      apply H1.
-    - apply tmap_subset_refl.
-Qed.
-
-Lemma stmts_tmap_cat :
-   forall (ss1 ss2 : HiFP.hfstmt_seq) (tmap_scope : ft_pmap * ft_pmap),
-      stmts_tmap tmap_scope (Qcat ss1 ss2) =
-      match stmts_tmap tmap_scope ss1 with
-      | Some tmap_scope' => stmts_tmap tmap_scope' ss2
-      | None => None
-      end.
-Proof.
-induction ss1.
-* simpl Qcat ; simpl stmts_tmap ; simpl.
-  by intro ; reflexivity.
-* simpl Qcat ; simpl stmts_tmap.
-  intros.
-  destruct (stmt_tmap tmap_scope h) ; last by reflexivity.
-  by apply IHss1.
-Qed.
-
-Fixpoint component_stmts_of (ss : HiFP.hfstmt_seq) : HiFP.hfstmt_seq :=
-match ss with
-| Qnil => ss
-| Qcons s ss' => Qcat (component_stmt_of s) (component_stmts_of ss')
-end
-with component_stmt_of (s : HiFP.hfstmt) : HiFP.hfstmt_seq :=
-match s with
-| Sskip
-| Sfcnct _ _
-| Sinvalid _ => Qnil ProdVarOrder.T
-| Swire _ _
-| Sreg _ _
-| Snode _ _
-| Smem _ _
-| Sinst _ _ => Qcons s (Qnil ProdVarOrder.T)
-| Swhen _ ss_true ss_false => Qcat (component_stmts_of ss_true) (component_stmts_of ss_false)
-end.
-
-Definition tmap_scope_subset (ts1 ts2 : ft_pmap * ft_pmap) : Prop :=
-fst ts1 = fst ts2 /\ tmap_subset (snd ts1) (snd ts2).
-
-Lemma stmts_tmap_components :
-   forall (ss : HiFP.hfstmt_seq) (tmap_scope1 tmap_scope2 : ft_pmap * ft_pmap),
-      tmap_subset (snd tmap_scope1) (fst tmap_scope1) ->
-      tmap_subset (snd tmap_scope2) (fst tmap_scope2) ->
-      tmap_scope_subset tmap_scope1 tmap_scope2 ->
-         match stmts_tmap tmap_scope1 ss, stmts_tmap tmap_scope2 (component_stmts_of ss) with
-         | Some result1, Some result2 =>
-              tmap_scope_subset result1 result2
-         | Some _, None => False
-         | _, _ => True
-         end
-with stmt_tmap_components :
-   forall (s : HiFP.hfstmt) (tmap_scope1 tmap_scope2 : ft_pmap * ft_pmap),
-      tmap_subset (snd tmap_scope1) (fst tmap_scope1) ->
-      tmap_subset (snd tmap_scope2) (fst tmap_scope2) ->
-      tmap_scope_subset tmap_scope1 tmap_scope2 ->
-         match stmt_tmap tmap_scope1 s, stmts_tmap tmap_scope2 (component_stmt_of s) with
-         | Some result1, Some result2 =>
-              tmap_scope_subset result1 result2
-         | Some _, None => False
-         | _, _ => True
-         end.
-Proof.
-* clear stmts_tmap_components.
-  induction ss.
-  + unfold component_stmts_of, stmts_tmap ; done.
-  + intros.
-    simpl stmts_tmap.
-    rewrite stmts_tmap_cat.
-    specialize stmt_tmap_components with (s := h) (tmap_scope1 := tmap_scope1) (tmap_scope2 := tmap_scope2).
-    generalize (stmt_tmap_subset h (fst tmap_scope1) (snd tmap_scope1) H) ;
-          intro ; rewrite -surjective_pairing in H2.
-    destruct (stmt_tmap tmap_scope1 h) as [tmap_scope1'|] ;
-          first rewrite (surjective_pairing tmap_scope1') in H2 ;
-          last by trivial.
-    generalize (stmts_tmap_subset (component_stmt_of h) (fst tmap_scope2) (snd tmap_scope2) H0) ;
-          intro ; rewrite -surjective_pairing in H3.
-    destruct (stmts_tmap tmap_scope2 (component_stmt_of h)) as [tmap_scope2'|] ;
-          first rewrite (surjective_pairing tmap_scope2') in H3.
-    - apply IHss, stmt_tmap_components ; try assumption.
-      * by apply (proj1 H2).
-      * by apply (proj1 H3).
-    - specialize IHss with (tmap_scope1 := tmap_scope1').
-      destruct (stmts_tmap tmap_scope1' ss) as [tmap_scope1''|] ; last by trivial.
-      apply stmt_tmap_components ; by assumption.
-* clear stmt_tmap_components.
-  intros.
-  destruct s ; simpl ; (try (by done)) ;
-        unfold tmap_scope_subset, tmap_subset in H1 ; destruct H1 ; try rewrite -H1.
-  + (* Swire *)
-    destruct (ft_find s (fst tmap_scope1)) ; simpl ; first by trivial.
-    unfold tmap_scope_subset ; split ; first by reflexivity.
-    simpl snd.
-    intro.
-    unfold ft_find, ft_add.
-    destruct (v == s) eqn: Hvs ; rewrite Hvs ; first by reflexivity.
-    by apply H2.
-  + (* Sreg *)
-    destruct (ft_find s (fst tmap_scope1)) ; simpl ; first by trivial.
-    destruct (reset h).
-    - unfold tmap_scope_subset ; split ; first by reflexivity.
-      simpl snd.
-      intro.
-      unfold ft_find, ft_add.
-      destruct (v == s) eqn: Hvs ; rewrite Hvs ; first by reflexivity.
-      by apply H2.
-    - destruct (type_of_expr h0 (snd tmap_scope1)) eqn: Hte0 ; last by trivial.
-      assert (type_of_expr h0 (snd tmap_scope2) = Some f).
-            generalize (type_of_expr_subset h0 (snd tmap_scope1) (snd tmap_scope2)) ; intro.
-            rewrite Hte0 in H3.
-            apply H3.
-            by exact H2.
-      rewrite H3.
-      destruct (type_of_expr h1 (snd tmap_scope1)) eqn: Hte1 ; last by trivial.
-      assert (type_of_expr h1 (snd tmap_scope2) = Some f0).
-            generalize (type_of_expr_subset h1 (snd tmap_scope1) (snd tmap_scope2)) ; intro.
-            rewrite Hte1 in H4.
-            apply H4.
-            by exact H2.
-      rewrite H4.
-      unfold tmap_scope_subset ; split ; first by reflexivity.
-      simpl snd.
-      intro.
-      unfold ft_find, ft_add.
-      destruct (v == s) eqn: Hvs ; rewrite Hvs ; first by reflexivity.
-      by apply H2.
-  + (* Snode *)
-    destruct (type_of_expr h (snd tmap_scope1)) as [[t p]|] eqn: Hte ; last by trivial.
-    assert (type_of_expr h (snd tmap_scope2) = Some (exist ftype_not_implicit_width t p)).
-          generalize (type_of_expr_subset h (snd tmap_scope1) (snd tmap_scope2)) ; intro.
-          rewrite Hte in H3.
-          apply H3.
-          by exact H2.
-    rewrite H3.
-    destruct (ft_find s (fst tmap_scope1)) ; simpl ; first by trivial.
-    unfold tmap_scope_subset ; split ; first by reflexivity.
-    simpl snd.
-    intro.
-    unfold ft_find, ft_add.
-    destruct (v == s) eqn: Hvs ; rewrite Hvs ; first by reflexivity.
-    by apply H2.
-  + (* Sfcnct *)
-    destruct (type_of_ref h (snd tmap_scope1)) ; last by trivial.
-    destruct (type_of_expr h0 (snd tmap_scope1)) ; last by trivial.
-    unfold tmap_scope_subset ; split ; first by exact H1.
-    by exact H2.
-  + (* Sinvalid *)
-    destruct (type_of_ref h (snd tmap_scope1)) ; last by trivial.
-    unfold tmap_scope_subset ; split ; first by exact H1.
-    by exact H2.
-  + (* Swhen *)
-    rename h0 into ss_true ; rename h1 into ss_false.
-    rewrite stmts_tmap_cat.
-    generalize (stmts_tmap_components ss_true tmap_scope1 tmap_scope2 H H0) ; intro.
-    generalize (stmts_tmap_subset ss_true (fst tmap_scope1) (snd tmap_scope1) H) ;
-          intro ; rewrite -surjective_pairing in H4.
-    destruct (stmts_tmap tmap_scope1 ss_true) as [[tmap_true tmap_scope_true]|] eqn: Hss_true ; last by trivial.
-    generalize (stmts_tmap_subset (component_stmts_of ss_true) (fst tmap_scope2) (snd tmap_scope2) H0) ;
-          intro ; rewrite -surjective_pairing in H5.
-    destruct (stmts_tmap tmap_scope2 (component_stmts_of ss_true)) as [[tmap_true' tmap_scope_true']|] eqn: Hss_true' ;
-          last by contradict H3 ; unfold tmap_scope_subset ; split ;
-                  first (by exact H1) ; exact H2.
-    assert (tmap_subset (snd tmap_scope1) tmap_true).
-          apply (tmap_subset_trans (fst tmap_scope1)) ; first (by exact H) ;
-          apply H4.
-    assert (tmap_scope_subset (tmap_true, snd tmap_scope1) (tmap_true', tmap_scope_true')).
-          split.
-          - simpl fst ; apply H3 ; exact (conj H1 H2).
-          - simpl snd ; apply (tmap_subset_trans (snd tmap_scope2)) ; first by exact H2.
-            by apply H5.
-    generalize (stmts_tmap_components ss_false (tmap_true, snd tmap_scope1) (tmap_true', tmap_scope_true') H6 (proj1 H5) H7) ; intro.
-    generalize (stmts_tmap_subset ss_false tmap_true (snd tmap_scope1) H6) ;
-          intro.
-    destruct (stmts_tmap (tmap_true, snd tmap_scope1) ss_false) as [[tmap_false tmap_scope_false]|] eqn: Hss_false ; last by trivial.
-    destruct (stmts_tmap (tmap_true', tmap_scope_true') (component_stmts_of ss_false)) as [[tmap_false' tmap_scope_false']|] eqn: Hss_false' ;
-          last by trivial.
-    split.
-    - simpl fst ; apply H8.
-    - simpl snd.
-      apply (tmap_subset_trans tmap_scope_false) ; first by apply H9.
-      apply H8.
-Qed.
+(*---------------------------------------------------------------------------*)
+(* Semantics of module                                                       *)
 
 Definition Sem (F : HiFP.hfmodule) (vm : module_graph_vertex_set_p.env) (ct : module_graph_connection_trees_p.env) : Prop :=
 (* The predicate returns True if G = (vm, ct) conforms to F.
@@ -1665,27 +1673,28 @@ Definition Sem (F : HiFP.hfmodule) (vm : module_graph_vertex_set_p.env) (ct : mo
    is that what you need? *)
 match F with
 | FInmod n pp ss =>
-    let pmap := ports_tmap pp in
-    match stmts_tmap (pmap, pmap) ss with
-    | Some (tmap, _) =>
-           (forall v1 v2: N,
-                match ft_find (v1, v2) tmap with
-                | Some (Gtyp _)
-                | None => True
-                | _ => (* (v1, N0) identifies an aggregate-type component;
-                          then there should not be any other component with the same v1 *)
-                       v2 = N0
-                    /\
-                       forall v2' : N, v2' <> N0 -> ft_find (v1, v2') tmap = None
-                end)
-        /\
-           exists (vm' : module_graph_vertex_set_p.env) (ct' : module_graph_connection_trees_p.env),
-                  Sem_frag_ports (module_graph_vertex_set_p.empty vertex_type)
-                                 (module_graph_connection_trees_p.empty def_expr)
-                                 pp vm' ct'
-               /\
-                  Sem_frag_stmts vm' ct' ss vm ct tmap
+    match ports_tmap pp vm with
+    | Some pmap =>
+        match stmts_tmap (pmap, pmap) ss vm with
+        | Some (tmap, _) =>
+               (forall v1 v2: N,
+                    match CEP.find (v1, v2) tmap with
+                    | Some (Gtyp _)
+                    | None => True
+                    | _ => (* (v1, v2) identifies an aggregate-type component;
+                              then there should not be any other component with the same v1 *)
+                           forall v2' : N, v2' <> v2 -> CEP.find (v1, v2') tmap = None
+                    end)
+            /\
+               exists (vm' : module_graph_vertex_set_p.env) (ct' : module_graph_connection_trees_p.env),
+                      Sem_frag_ports (module_graph_vertex_set_p.empty vertex_type)
+                                     (module_graph_connection_trees_p.empty def_expr)
+                                     pp vm' ct' tmap
+                   /\
+                      Sem_frag_stmts vm' ct' ss vm ct tmap
+        | None => False
+        end
     | None => False
     end
 | FExmod _ _ _ => False
-end.
+ end.
